finish new non-flat reduction to Clique; refactoring

theories/L/Complexity/Problems/Clique.v
@@ -1,283 +1,44 @@
-From Undecidability.L Require Import L.
-From Undecidability.L.Tactics Require Import LTactics ComputableTactics.
-From Undecidability.L.Datatypes Require Import LProd LTerm LNat Lists LOptions.
-From Undecidability.L.Complexity Require Import NP Synthetic Monotonic LinTimeDecodable Tactics Problems.LGraph.
-From Undecidability.L.Functions Require Import Size.
+From PslBase Require Import FinTypes. 
+From Undecidability.L.Complexity.Problems Require Import UGraph. 
+Require Import Lia.
 
+Section fixGraph. 
+  Variable (g : UGraph). 
+  Notation V := (V g).
+  Notation E := (@E g).
 
-(* k-Clique: duplicate-free list of k nodes such that all pairwise-distinct nodes are connected *)
-Inductive isLClique (g : Lgraph) : list Lnode -> nat -> Prop :=
-| isLCliqueB : isLClique g [] 0
-| isLCliqueS (cl : list Lnode) (node : Lnode) (k : nat) : isLClique g cl k ->
-    (not (node el cl)) -> Lgraph_node_in_dec g node = true -> (forall (node' : Lnode), node' el cl -> Lgraph_edge_in_dec g node node' = true) -> isLClique g (node :: cl) (S k).                                                     
+  Definition isClique (l : list V) := (forall v1 v2, v1 el l -> v2 el l -> v1 <> v2 -> E (v1, v2)) /\ dupfree l. 
+  Definition isKClique k (l : list V) := |l| = k /\ isClique l. 
 
-Lemma isLClique_node_in (g : Lgraph) (k : nat) (cl : list Lnode) : isLClique g cl k -> forall n, n el cl -> Lgraph_node_in_dec g n = true. 
-Proof.
-  induction 1. 
-  -intros n [].
-  - intros n [-> | H3]. apply H1. now apply IHisLClique. 
-Qed. 
+  Inductive indKClique : nat -> list V -> Prop := 
+    | indKCliqueNil : indKClique 0 []
+    | indKCliqueS L v k : indKClique k L -> not (v el L) -> (forall v', v' el L -> E (v, v')) -> indKClique (S k) (v :: L). 
+  Hint Constructors indKClique.
 
-Lemma isLClique_length (g : Lgraph) (k : nat) (cl : list Lnode) : isLClique g cl k -> k = (|cl|).
-Proof. induction 1; now cbn. Qed. 
-
-Definition isLClique_explicit (g : Lgraph) (cl : list Lnode) (k : nat) :=
-  |cl| = k /\ dupfree cl /\ (forall n, n el cl -> Lgraph_node_in_dec g n = true) /\ (forall (n m : nat), n <> m -> n el cl -> m el cl -> Lgraph_edge_in_dec g n m = true).
-Lemma isLClique_explicit_correct (g : Lgraph) (cl : list Lnode) (k : nat) :
-  isLClique g cl k <-> isLClique_explicit g cl k. 
-Proof.
-  split.
-  - induction 1.
-    + split; try split. constructor. split. intros n []. intros _ n m _ []. 
-    + destruct IHisLClique as [IH1 [IH2 [IH3 IH4]]]. split; try split. now rewrite <- IH1.  
-      now constructor. split.
-      -- intros n [-> | H3]. apply H1. now apply IH3. 
-      -- intros n m H5 [-> | F1] [-> | F2].  
-         * congruence.
-         * now apply H2. 
-         * destruct g as (nodes & e).
-           destruct (Lgraph_edge_in_dec_correct (nodes, e) m n) as [H6 _].
-           specialize (H6 (H2 n F1)). apply (Lgraph_edge_in_dec_correct (nodes, e) n m). tauto. 
-         * now apply IH4.  
-  - revert k. induction cl.
-    * intros k H. destruct H as [H1 [H2 [H3 H4]]]. cbn in H1; rewrite <- H1. constructor.
-    * intros [] [H1 [H2 [H3 H4]]]. 
-      -- cbn in H1. congruence. 
-      -- constructor. apply IHcl. split. cbn in H1. lia. 
-         split. now inv H2.
-         split. intros m H. now apply H3. 
-         intros m1 m2 F1 F2 F3. now apply H4.
-         now inv H2. now apply H3. 
-         intros m H. apply H4. inv H2. now intros ->. now left. now right. 
-Qed. 
-
-(** *TODO: include well-formedness*)
-Definition LClique (input : Lgraph * nat) :=
-  let (g, k) := input in exists cl, @isLClique g cl k. 
-
-Definition LClique_verifier (input : Lgraph * nat) (cert : list Lnode) :=
-  let (g, k) := input in isLClique g cert k. (*this includes that l is short enough*)
-
-Lemma size_nat_enc_mono (n  :nat) (m : nat) :
-  n <= m -> size (enc n) <= size(enc m). 
-Proof. 
-  intros H; repeat rewrite size_nat_enc. lia. 
-Qed. 
-
-Fixpoint connectedb (g : Lgraph) (cl : list Lnode) :=
-  match cl with [] => true
-           | (n :: cl) => forallb (Lgraph_edge_in_dec g n) cl && connectedb g cl
-  end. 
-
-(*TODO: maybe factor out the 2nd induction*)
-Lemma connectedb_correct (g : Lgraph) (cl : list Lnode) : dupfree cl -> connectedb g cl = true <-> forall u v, u <> v -> u el cl -> v el cl -> Lgraph_edge_in_dec g u v = true. 
-Proof. 
-  intros F0. 
-  destruct g. induction cl. 
-  + cbn. tauto. 
-  + split; cbn.
-  - intros H%andb_prop; destruct H as [F1 F2]. intros u v neq [H1 | H1] [H2 | H2].
-    * congruence.
-    * rewrite H1 in *; clear H1.
-      apply (proj1 (forallb_forall (Lgraph_edge_in_dec (n, l) u) cl) F1 v H2 ).
-    * rewrite H2 in *; clear H2.
-      specialize (proj1 (forallb_forall (Lgraph_edge_in_dec (n, l) v) cl) F1 u H1) as H0.
-      apply (Lgraph_edge_in_dec_correct (n, l)). apply (Lgraph_edge_in_dec_correct (n, l)) in H0. tauto.
-    * inv F0. apply IHcl; tauto. 
-  - intros H. apply utils.andb_and; split.
-    2: {apply IHcl. firstorder. now inv F0. firstorder. }
-    clear IHcl. induction cl. reflexivity. 
-    cbn. apply utils.andb_and; split.
-    2: {inv F0. inv H3. assert (dupfree (a :: cl)). constructor. firstorder. apply H5. apply IHcl;firstorder. }
-    apply H. inv F0. 1-2: firstorder. right; left; reflexivity. 
-Qed. 
-
-Definition LClique_verifierb (g : Lgraph) (k : nat) (cl : list Lnode) :=
-  forallb (Lgraph_node_in_dec g) cl && dupfreeb Nat.eqb cl && connectedb g cl && Nat.eqb (|cl|) k.   
-
-Definition nat_eqb_correct := (fun a b => conj (proj2 (Nat.eqb_eq a b)) (proj1 (Nat.eqb_eq a b))). 
-
-Lemma LClique_verifierb_correct (g : Lgraph) (k : nat) (cl : list Lnode) :
-  reflect (isLClique g cl k) (LClique_verifierb g k cl). 
-Proof.
-  destruct LClique_verifierb eqn:H; constructor; rewrite isLClique_explicit_correct. 
-  - split; try split; try split; unfold LClique_verifierb in H; simp_bool.
-    3: now rewrite forallb_forall in H0.
-    now apply nat_eqb_correct. 
-    all: rewrite <- (reflect_iff (dupfree cl) (dupfreeb Nat.eqb cl) (dupfreeb_correct nat_eqb_correct cl)) in H3.
-    assumption. now rewrite connectedb_correct in H2. 
-  - intros [H1 [H2 [H3 H4]]]. unfold LClique_verifierb in H. simp_bool.
-    + now rewrite <- forallb_forall in H3. 
-    + now rewrite -> (reflect_iff (dupfree cl) (dupfreeb Nat.eqb cl) (dupfreeb_correct nat_eqb_correct cl)) in H2.
-    + now rewrite <- connectedb_correct in H4. 
-    + now apply nat_eqb_correct in H1. 
-Qed. 
-
-From Undecidability.L.Complexity Require Import PolyBounds ONotation Monotonic. 
-
-(*extraction of needed functions and derivation of runtime bounds in terms of encoding size*)
-
-Fixpoint connectedb_time (g : Lgraph) (cl : list Lnode) :=
-  let (n, e) := g in 
-  match cl with [] => 4
-              | (cl :: cls) => forallb_time
-  (fun (v : Lnode) (_ : unit) =>
-  (list_in_decb_time pair_eqb_nat_time e (cl, v) +
-    list_in_decb_time pair_eqb_nat_time e (v, cl) + 26, tt)) cls + 19 + connectedb_time g cls
-            end. 
-
-Instance term_connectedb : computableTime' connectedb (fun g _ => (5, fun cl _ => (connectedb_time g cl, tt))).
-Proof.
-  extract. 
-  solverec. 
-Qed. 
-
-Lemma connectedb_time_bound : exists (f : nat -> nat), (forall (g : Lgraph) (cl : list Lnode), connectedb_time g cl <= f (size(enc g) + size(enc cl))) /\ inOPoly f /\ monotonic f.
-Proof.
-  (*bound the running time of each step*)
-  (*the step function used with forall is not closed, therefore the running time function needs to explicitly capture the needed *)
-  (*environment variables *)
-  pose (forallb_step_time := fun (env : Lgraph * Lnode) => let (g, a) := env in (fun (v : nat) (_ : unit) => (Lgraph_edge_in_dec_time g a v, tt))).
-  pose (step_time := fun (g : Lgraph) cl cls => forallb_time (forallb_step_time (g, cl)) cls + 19).
-
-  (*We would like to get a polynomial in g and the clique cl*)
-  assert (exists (f : nat -> nat), (forall (g : Lgraph) (cl : list Lnode) (a : Lnode) (cls: list Lnode),
-             a el cl -> subsequence cls cl -> step_time g a cls <= f(size(enc g) + size(enc cl)))
-             /\ inOPoly f /\ monotonic f) as (f' & H1 & H2 & H3).
-  {
-    destruct (Lgraph_edge_in_dec_time_bound) as (f__edgeIn & F1 & F2 & F3).
-    (*In order to instantiate forallb_time_bound_env, we need to prove another result first*)
-    assert (exists (f' : nat -> nat), (forall a env, fst (forallb_step_time env a tt) <= f'(size (enc a) + size(enc env))) /\ inOPoly f' /\ monotonic f').
-    {
-      exists f__edgeIn. split.
-      - intros node (e & node'). unfold forallb_step_time. cbn. rewrite F1. setoid_rewrite size_prod at 2; cbn[fst snd].
-        unfold monotonic in F3; apply F3. lia. 
-      - tauto. 
-    }
-    destruct (forallb_time_bound_env H) as (f__forall & E1 & E2 & E3).
-    evar (f : nat -> nat). exists f. split.
-    - intros. unfold step_time. rewrite E1. rewrite size_prod; cbn [fst snd]. 
-      unfold monotonic in E3. rewrite E3 with (x' := size(enc g) + 2 * size (enc cl)  + 4). 
-      instantiate (f := fun n => f__forall (2 * n + 4) + 19). subst f. cbn. 
-      rewrite <- Nat.add_le_mono_r. apply E3. lia. 
-      rewrite (list_subsequence_size_bound H1). 
-      rewrite (list_el_size_bound H0). lia. 
-    - subst f; split; smpl_inO. apply inOPoly_comp; smpl_inO. 
-  }
-
-  evar (f : nat -> nat). exists f. split.
-  - intros g cl. unfold connectedb_time.
-    instantiate (f:= fun n => 4 + f' n * n). subst f.
-    destruct g as (n, e). induction cl.
-    + lia.
-    + rewrite IHcl. specialize (H1 (n, e) (a::cl) a cl).
-      unfold step_time, forallb_step_time, Lgraph_edge_in_dec_time in H1. rewrite H1.
-      3: exists [a], []; firstorder.  2: now left.
-      rewrite list_size_cons at 3.
-      unfold monotonic in H3.
-      rewrite H3 with (x:= size(enc(n, e)) + size(enc(cl)))(x' := size(enc(n, e)) + size(enc(a::cl))).
-      solverec.
-      rewrite (list_size_cons); lia. 
-  - subst f; split; smpl_inO. 
-Qed. 
-
-Definition Lclique_verifierb_time (g : Lgraph) (k:nat) (cl : list Lnode):= forallb_time (fun n _ => (33 + 14 * n, tt)) cl
-  + dupfreeb_time (fun x _ => (5, fun y _ => (min x y * 17 + 9, tt))) cl
-  + connectedb_time g cl + 11 * (|cl|) + 17 * min (|cl|) k + 53.
-
-Instance term_LClique_verifierb : computableTime' LClique_verifierb (fun g _ => (1, fun k _ => (1, fun cl _ => (Lclique_verifierb_time g k cl, tt)))). 
-Proof.
-  extract. 
-  solverec. unfold Lclique_verifierb_time. solverec. 
-Qed. 
-
-Lemma Lclique_verifierb_time_bound : exists (f : nat -> nat) , (forall (g: Lgraph) (k : nat) (cl : list Lnode), Lclique_verifierb_time g k cl <= f(size(enc g) + size(enc cl))) /\ inOPoly f /\ monotonic f. 
-Proof.
-  assert (exists (f : nat -> nat), (forall (a : Lnode), fst((fun n _ => (33 + 14 * n, tt)) a tt) <= f(size(enc a))) /\ inOPoly f /\ monotonic f).
-  {
-    evar (f : nat -> nat); exists f; split.
-    - intros a. cbn -[Nat.mul Nat.add]. rewrite size_nat_enc. 
-      instantiate (f := fun n => 4 * n + 17); subst f; lia. 
-    - split; subst f; smpl_inO. 
-  }
-  destruct (forallb_time_bound H) as (f__forall & H1 & H2 & H3); clear H.
-
-  assert (exists (f : nat -> nat), (forall (a b : nat), callTime2 (fun x _ => (5, fun y _ => (min x y * 17 + 9, tt))) a b <= f(size(enc a) + size(enc b))) /\ inOPoly f /\ monotonic f).
-  {
-    evar (f : nat -> nat). exists f; split.
-    - intros a b. cbn -[Nat.add]. rewrite Nat.le_min_r. solverec.
-      instantiate (f := fun n => 17 * n + 14). subst f. 
-      specialize size_nat_enc_r with (n:= b). lia.
-    - split; subst f; smpl_inO.
-  }
-  destruct (dupfreeb_time_bound H) as (f__dupfree & F1 & F2 & F3); clear H.
-
-  destruct (connectedb_time_bound) as (f__connected & E1 & E2 & E3).
-
-  evar (f : nat -> nat). exists f. split.
-  - intros g k cl. unfold Lclique_verifierb_time. 
-    rewrite H1, F1, E1. rewrite Nat.le_min_l. repeat rewrite list_size_length.
-    unfold monotonic in H3, F3.
-    rewrite H3 with (x':= size(enc g) + size(enc cl)) by lia.
-    rewrite F3 with (x':= size(enc g) + size(enc cl)) by lia. 
-    instantiate (f := fun n => f__connected n + f__forall n + f__dupfree n + 28 * n + 53); subst f.
-    solverec.
-  - subst f; split; smpl_inO.
-Qed.
-
-Lemma clique_inNP : inNP LClique. 
-Proof.
-  apply (inNP_intro) with (R:= LClique_verifier).
-  1: { apply linDec_polyTimeComputable. }
-  3 : {
-    intros [g k]; split.
-    - destruct g. intros (cert & H1). exists cert. easy.  
-    - intros (cert & H). now exists cert. 
-  }
-  2 : {
-    evar (f' : nat -> nat). 
-    exists f'. split. 2: split. 
-    2: {
-      intros [g k] cert H. cbn in H.
-      assert (k = (|cert|)) by (now apply isLClique_length with (g:= g)).
-      rewrite H0 in *; clear H0 k. rewrite size_prod; cbn [fst snd].
-      rewrite size_nat_enc. rewrite size_list.
-      (*LHS is in O(max_node * |cert|) *)
-      specialize (isLClique_node_in H) as H2. 
-      unfold Lgraph_node_in_dec in H2. destruct g.
-      assert (sumn (map (fun (x : nat ) => size (enc x) + 5) cert) <= (size(enc n) + 5) * (|cert|)).
-      - induction cert. cbn; lia.
-        cbn. assert (a <= n).
-        { assert (Lgraph_node_in_dec (n, l) a = true ).
-          apply isLClique_node_in with (k:= |a::cert|) (cl:= a::cert); easy.
-          cbn in H0. destruct n. congruence. dec_bool. lia.
-        }
-        apply size_nat_enc_mono in H0. rewrite H0. rewrite IHcert. solverec.
-        now inv H. firstorder. 
-      - rewrite H0. rewrite size_prod with (w := (n, l)); cbn [fst snd].
-        instantiate (f' := fun n => 4 * n * n). subst f'.
-        solverec.
-    }
-    all: (subst f'; smpl_inO).
-  }
-
-  destruct (Lclique_verifierb_time_bound) as (f' & H1 & H2 & H3).
-  evar (f : nat -> nat). exists f. split; try split.
-  - exists (fun inp => match inp with ((g, k), cert) => LClique_verifierb g k cert end).
+  (** an alternative inductive characterisation *)
+  Lemma indKClique_iff k L: isKClique k L <-> indKClique k L. 
+  Proof. 
     split.
-    + constructor. extract. solverec.
-      repeat (rewrite size_prod; cbn [fst snd]).
-      rewrite H1. rewrite size_prod; cbn [fst snd].
-      instantiate (f:= fun n => f'(n) + 11). subst f.
-      cbn. unfold monotonic in H3. rewrite H3 at 1.
-      2 : {
-        assert (size(enc a) + size(enc b1) + 4 + size(enc b) <= size(enc a) + size(enc b1) + 4 + size(enc b0) + 4+ size(enc b) + 4).
-        2: apply H. lia.
-      }
-      reflexivity. 
-  + intros [[g k] b]. specialize (LClique_verifierb_correct g k) as H4.
-    destruct (reflect_iff (isLClique g b k) (LClique_verifierb g k b)) as (F1 & F2). apply H4.
-    split; cbn; tauto. 
- - subst f; smpl_inO. 
- - subst f; smpl_inO. 
-Qed. 
+    - intros [H1 [H2 H3]]. revert L H1 H2 H3. induction k; intros. 
+      + destruct L; cbn in H1; [ eauto | congruence].
+      + destruct L; cbn in *; [congruence | ].
+        constructor.
+        * apply IHk; [lia | intros; apply H2; eauto | now inv H3].
+        * now inv H3. 
+        * intros v' Hel. apply H2; [eauto | eauto | ]. inv H3. intros ->. congruence.
+    - induction 1 as [ | ? ? ? ? IH]. 
+      + split; [ | split]; [now cbn | intros ? ? [] | constructor].
+      + destruct IH as (IH1 & IH2 & IH3). split; [ | split].
+        * cbn. lia.
+        * intros v1 v2 [-> | H2] [-> | H3] H4; try congruence.
+          -- now apply H1. 
+          -- apply E_symm. now apply H1. 
+          -- now apply IH2. 
+        * now constructor.
+  Qed. 
+End fixGraph. 
+  
+Definition Clique (i : UGraph * nat) := let (g, k) := i in exists l, @isKClique g k l.  
+
+
+
