theories/L/Complexity/Problems/SAT.v
@@ -1,9 +1,11 @@
-From Undecidability.L Require Import L.
-From Undecidability.L.Tactics Require Import LTactics ComputableTactics.
-From Undecidability.L.Datatypes Require Import LProd LTerm LNat Lists LOptions.
-From Undecidability.L.Complexity Require Import NP Synthetic Monotonic Tactics PolyBounds MorePrelim.
-From Undecidability.L.Functions Require Import Size.
+From Undecidability.L.Complexity.Cook Require Import Prelim.
+From Undecidability.L.Complexity.Problems Require Export SharedSAT.
+Require Import Lia. 
+From Undecidability.L.Datatypes Require Import LLists. 
 
+From Undecidability.L.Tactics Require Import LTactics GenEncode.
+From Undecidability.L.Datatypes Require Import  LProd LOptions LBool LLNat LLists LUnit.
+From Undecidability.L.Complexity Require Import PolyBounds. 
 
 (*Conjunctive normal forms (need not be canonical)*)
 Notation var := (nat) (only parsing). 
@@ -12,703 +14,923 @@ Notation clause := (list literal) (only parsing).
 Notation cnf := (list clause) (only parsing).
 
 
-(*Bounds on the number of used variables*)
+(*Assignments as lists of natural numbers: contain the indices of variables that are mapped to true *)
+Notation assgn := (list nat). 
+Implicit Types (a : assgn) (N : cnf) (C : clause) (l :literal).
+
+Definition evalLiteral a l : bool := match l with
+  | (s, v) => Bool.eqb (evalVar a v) s 
+end. 
+
+(*Empty disjunction evaluates to false*)
+Definition evalClause_step a lit acc := orb acc (evalLiteral a lit). 
+Definition evalClause a C : bool := fold_right (evalClause_step a) false C. 
+
+(*Empty conjunction evaluates to true *)
+Definition evalCnf_step a cl acc := andb acc (evalClause a cl). 
+Definition evalCnf a N : bool := fold_right (evalCnf_step a) true N. 
+
+(*more helpful properties *)
+(*a characterisation of one processing step of evalClause *)
+Lemma evalClause_step_inv a C l b : 
+  evalClause a (l::C) = b <-> exists b1 b2, evalClause a C = b1 /\ evalLiteral a l = b2 /\ b = b1 || b2.
+Proof.
+  cbn. split; intros. 
+  - rewrite <- H. eauto. 
+  - destruct H as (b1 & b2 & <- & <- & ->). eauto.
+Qed. 
+
+Lemma evalCnf_step_inv a N C b : 
+  evalCnf a (C :: N) = b <-> exists b1 b2, evalCnf a N = b1 /\ evalClause a C = b2 /\ b = b1 && b2. 
+Proof. 
+  cbn. split; intros. 
+  - rewrite <- H. eauto. 
+  - destruct H as (b1 & b2 & <- & <- & ->). eauto.
+Qed. 
+
+Lemma evalLiteral_var_iff a b v : 
+  evalLiteral a (b, v) = true <-> evalVar a v = b. 
+Proof. 
+  unfold evalLiteral. destruct b, evalVar; cbn; firstorder.
+Qed. 
+
+Lemma evalClause_literal_iff a C : 
+  evalClause a C = true <-> (exists l, l el C /\ evalLiteral a l = true). 
+Proof.
+  induction C; cbn. 
+  - split; [ congruence | firstorder].
+  - split. 
+    + intros [H1 | H2]%orb_true_iff.
+      * apply IHC in H1 as (l & H1 & H2). eauto.
+      * exists a0; eauto.
+    + intros (l & [-> | H1] & H2). 
+      * unfold evalClause_step. now rewrite H2, orb_true_r. 
+      * fold (evalClause a C). erewrite (proj2 IHC); [easy | eauto].
+Qed. 
+
+Corollary evalClause_app a C1 C2 : 
+  evalClause a (C1 ++ C2) = true <-> (evalClause a C1 = true \/ evalClause a C2 = true). 
+Proof. 
+  rewrite !evalClause_literal_iff. setoid_rewrite in_app_iff. firstorder.
+Qed.
+
+Lemma evalCnf_clause_iff a N : 
+  evalCnf a N = true <-> (forall C, C el N -> evalClause a C = true). 
+Proof. 
+  induction N; cbn. 
+  - firstorder. 
+  - split. 
+    + intros (H1 & H2)%andb_true_iff. intros C [-> | H3]; [easy | ].
+      fold (evalCnf a N) in H1. eapply (proj1 IHN) in H1; eauto.
+    + intros H. unfold evalCnf_step. rewrite (H a0 (or_introl eq_refl)), andb_true_r. 
+      apply IHN; eauto.
+Qed. 
+
+Corollary evalCnf_app_iff a N1 N2 : 
+  evalCnf a (N1 ++ N2) = true <-> (evalCnf a N1 = true /\ evalCnf a N2 = true). 
+Proof. 
+  rewrite !evalCnf_clause_iff. setoid_rewrite in_app_iff. firstorder.
+Qed.
+
+Definition satisfies a N := evalCnf a N = true.
+Definition SAT N : Prop := exists (a : assgn), satisfies a N. 
+
+Lemma evalLiteral_assgn_equiv a1 a2 l : a1 === a2 -> evalLiteral a1 l = evalLiteral a2 l. 
+Proof. 
+  intros [H1 H2]. destruct l as (b & v). unfold evalLiteral. destruct (evalVar a1 v) eqn:Hev1. 
+  - apply (evalVar_monotonic H1) in Hev1. easy.
+  - destruct (evalVar a2 v) eqn:Hev2; [ | easy]. 
+    apply (evalVar_monotonic H2) in Hev2. congruence. 
+Qed.
+
+Lemma evalClause_assgn_equiv a1 a2 C : a1 === a2 -> evalClause a1 C = evalClause a2 C. 
+Proof. 
+  intros H. enough (evalClause a1 C = true <-> evalClause a2 C = true).
+  - destruct evalClause; destruct evalClause; firstorder; easy. 
+  - rewrite !evalClause_literal_iff. now setoid_rewrite (evalLiteral_assgn_equiv _ H). 
+Qed.
+
+Lemma evalCnf_assgn_equiv a1 a2 N : a1 === a2 -> evalCnf a1 N = evalCnf a2 N. 
+Proof. 
+  intros H. enough (evalCnf a1 N = true <-> evalCnf a2 N = true). 
+  - destruct evalCnf; destruct evalCnf; firstorder; easy.
+  - rewrite !evalCnf_clause_iff. now setoid_rewrite (evalClause_assgn_equiv _ H).
+Qed. 
+
+(** Bounds on the number of used variables*)
 Inductive varBound_clause (n : nat) : clause -> Prop :=
   | varBound_clauseB : varBound_clause n []
-  | varBound_clauseS : forall b k c, k < n -> varBound_clause n c -> varBound_clause n ((b, k) :: c).  
+  | varBound_clauseS : forall b v C, v < n -> varBound_clause n C -> varBound_clause n ((b, v) :: C).  
 
 Inductive varBound_cnf (n : nat) : cnf -> Prop :=
    | varBound_cnfB : varBound_cnf n [] 
-   | varBound_cnfS : forall cl c, varBound_clause n cl -> varBound_cnf n c -> varBound_cnf n (cl :: c).  
+   | varBound_cnfS : forall C N, varBound_clause n C -> varBound_cnf n N -> varBound_cnf n (C :: N).  
 
-Lemma varBound_clause_iff (n : nat) (c : clause) : varBound_clause n c <-> forall (s : bool) (k : nat), (s, k) el c -> k < n.
+Hint Constructors varBound_clause varBound_cnf. 
+
+Lemma varBound_clause_iff (n : nat) C : varBound_clause n C <-> forall (s : bool) v, (s, v) el C -> v < n.
 Proof.
   split.
   - induction 1.
-    + intros s k []. 
-    + intros s k0 [H1 | H1].
+    + intros s v []. 
+    + intros s v0 [H1 | H1].
       * inv H1. now apply H. 
       * now apply IHvarBound_clause with (s := s). 
-  - induction c.
+  - induction C.
     + intros. constructor. 
     + intros. destruct a. constructor.
       * apply H with (s := b). firstorder.  
-      * apply IHc. firstorder.  
+      * apply IHC. firstorder.  
 Qed. 
 
-Lemma varBound_cnf_iff (n : nat) (c : cnf) : varBound_cnf n c <-> forall (cl : clause), cl el c -> varBound_clause n cl.
+Lemma varBound_cnf_iff (n : nat) N : varBound_cnf n N <-> forall C, C el N -> varBound_clause n C.
 Proof.
   split.
   - induction 1. 
-    + intros cl [].
-    + intros cl' [-> |Hel]. assumption. now apply IHvarBound_cnf. 
-  - intros H. induction c; constructor.
+    + intros C [].
+    + intros C' [-> |Hel]. assumption. now apply IHvarBound_cnf. 
+  - intros H. induction N; constructor.
     + now apply H. 
-    + apply IHc. firstorder.
+    + apply IHN. firstorder.
 Qed. 
 
-Lemma varBound_clause_monotonic (c : clause) (n n' : nat) : n <= n' -> varBound_clause n c -> varBound_clause n' c. 
+Lemma varBound_clause_monotonic C (n n' : nat) : n <= n' -> varBound_clause n C -> varBound_clause n' C. 
 Proof. intros H1 H2. induction H2. constructor. constructor. lia. auto. Qed. 
 
-Lemma varBound_cnf_monotonic (c : cnf) (n n' : nat) : n <= n' -> varBound_cnf n c -> varBound_cnf n' c.
+Lemma varBound_cnf_monotonic N (n n' : nat) : n <= n' -> varBound_cnf n N -> varBound_cnf n' N.
 Proof.
   intros H1 H2. induction H2; constructor.
   now apply varBound_clause_monotonic with (n:= n). assumption. 
 Qed.
 
-(*Assignments as lists of natural numbers: variable i is mapped to value list[i] *)
-Notation assgn := (list bool). 
-
-Definition evalLiteral (a : assgn) (l : literal) : option bool := match l with
-  | (s, v) => match nth_error a v with
-               | Some value => Some (Bool.eqb s value)
-               | _ => None
-  end 
-end. 
-
-
-(*foldr, but on option values. If the step function ever returns None, this pins the result to None *)
-Definition fold_rightOption (A B : Type) (f : B -> A -> option A) := fix rec (acc : option A) (l : list B) : option A :=
-  match l with
-    | [] => acc
-    | (l :: ls) => match rec acc ls with
-                   | None => None
-                   | Some acc => f l acc 
-                  end
-  end. 
-
-(*Empty disjunction evaluates to false*)
-Definition evalClause (a : assgn) (l : clause) : option bool := 
-  fold_rightOption (fun lit acc => match evalLiteral a lit with Some v => Some(orb acc v) | _ => None end) (Some false) l.  
-
-(*Empty conjunction evaluates to true *)
-Definition evalCnf (a : assgn) (l : cnf) : option bool :=
-  fold_rightOption (fun cl acc => match evalClause a cl with Some v => Some(andb acc v) | _ => None end) (Some true) l.
-
-(*Correctness: if the assignment a assigns a value to each used variable, then the result will be a Some _ *)
-
-Lemma evalLiteral_correct (b : bool) (k : nat) (a : assgn) (n : nat) : k < n -> |a| >= n -> exists v, evalLiteral a (b, k) = Some v. 
+Lemma varBound_cnf_app N1 N2 (n : nat) : varBound_cnf n N1 /\ varBound_cnf n N2 <-> varBound_cnf n (N1 ++ N2).
 Proof.
-  intros H1 H2. unfold evalLiteral. destruct nth_error eqn:H3. eauto.
-  destruct (nth_error_None a k) as [F1 _]. apply F1 in H3.
-  omega. 
+  induction N1; cbn. 
+  - split; [ tauto | intros H; split; eauto  ]. 
+  - split. 
+    + intros (H1 & H2). inv H1. constructor; [eauto | now apply IHN1].
+    + intros H. inv H. apply IHN1 in H3 as (H3 & H4). split; eauto. 
 Qed. 
 
-Lemma evalClause_correct (l : clause) (a : assgn) (n : nat): varBound_clause n l -> |a| >= n -> exists v, evalClause a l = Some v. 
-Proof. 
-  intros H1; induction H1. 
-  - intros; cbn. now exists false.
-  - intros. unfold evalClause, fold_rightOption. 
-    destruct (IHvarBound_clause H0) as [v' H3]. unfold evalClause, fold_rightOption in H3. rewrite H3.
-    destruct (evalLiteral_correct b H H0) as [v H2]. rewrite H2. exists (v' || v); auto.
-Qed. 
+(*size of CNF in terms of number of operators *)
+Definition size_clause C := length C. (*we should subtract 1 here, but this would only complicate things *)
+Definition size_cnf N := sumn (map size_clause N) + length N. 
 
-Lemma evalCnf_correct (l : cnf) (a : assgn) (n : nat): varBound_cnf n l -> |a| >= n -> exists v, evalCnf a l = Some v. 
+Lemma size_clause_app C1 C2 : size_clause (C1 ++ C2) = size_clause C1 + size_clause C2. 
 Proof. 
-  intros H1; induction H1. 
-  - intros. cbn. now exists true.
-  - intros. cbn. destruct (evalClause_correct H H0) as [v H2]. 
-    rewrite H2. destruct (IHvarBound_cnf H0) as [v' H3]. unfold evalCnf in H3. rewrite H3.
-    exists (v' && v); auto.
+  unfold size_clause. now rewrite app_length. 
 Qed.
 
-
-(*if a formula evaluates, the variable indices are bounded by the assignment length*)
-Lemma evalLiteral_varBound (n: nat) (sign : bool) (a : assgn) : (exists v, evalLiteral a (sign, n) = Some v) -> n < |a|. 
+Lemma size_cnf_app N1 N2 : size_cnf (N1 ++ N2) = size_cnf N1 + size_cnf N2. 
 Proof. 
-  intros [v H]. unfold evalLiteral in H. destruct (nth_error a n) eqn:H1.
-  apply nth_error_Some. congruence.
-  discriminate H. 
+  unfold size_cnf. rewrite map_app, sumn_app, app_length. lia.
 Qed. 
 
-Lemma evalClause_varBound (l : clause) (a : assgn): (exists v, evalClause a l = Some v) -> varBound_clause (|a|) l. 
+(** * Verifier for SAT*)
+(** The certificate is a satisfying assignment.
+  The assignment needs to be short enough and must not contain variables not occuring in the CNF.
+*)
+
+(*produce a list (possibly containing duplicates) of variables occuring in a CNF *)
+Definition varsOfLiteral (l : literal) := match l with (_, v) => [v] end. 
+Definition varsOfClause (C : clause) := concat (map varsOfLiteral C).
+Definition varsOfCnf (N : cnf) := concat (map varsOfClause N).
+
+Lemma varsOfLiteral_correct l v : v el varsOfLiteral l <-> exists b, l = (b, v). 
 Proof. 
-  induction l; try constructor. 
-  destruct a0 as [b0 v0]. constructor.
-  - destruct H as [v H]. unfold evalClause, evalClause, fold_rightOption in H.
-    destruct (evalLiteral a (b0, v0)) eqn:H1.
-    + apply evalLiteral_varBound with (sign := b0). exists b; apply H1. 
-    + change (match evalClause a l with | Some _ | _ => None end = Some v) in H.
-      destruct (evalClause a l); congruence. 
-  - apply IHl. destruct H as (v & H). 
-    unfold evalClause, fold_rightOption in H.
-    change (match evalClause a l with |Some acc => match evalLiteral a (b0, v0) with | Some v => Some (acc || v) | None => None end | None => None end = Some v) in H.
-    destruct (evalClause a l).
-    * now exists b.
-    * congruence. 
+  unfold varsOfLiteral; destruct l; cbn. split. 
+  - intros [-> | []]. now exists b.
+  - intros [? H]. inv H. easy.
 Qed. 
 
-Lemma evalCnf_varBound (l : cnf) (a : assgn): (exists v, evalCnf a l = Some v) -> varBound_cnf (|a|) l. 
+Lemma varsOfClause_correct C v : v el varsOfClause C <-> exists l, l el C /\ v el varsOfLiteral l. 
 Proof. 
-  induction l; try constructor. 
-  - destruct H as [v H]. cbn in H. destruct (evalClause a a0) eqn:H1.
-    + apply evalClause_varBound. rewrite H1; eauto. 
-    + destruct (fold_rightOption) in H; congruence.  
-  - cbn in H. destruct (evalClause a a0) eqn:H1.
-    + apply IHl. unfold evalCnf. destruct (fold_rightOption) eqn:H2; [ |destruct H; congruence ]. now exists b0. 
-    + destruct fold_rightOption in H; destruct H; congruence.   
+  unfold varsOfClause. now rewrite in_concat_map_iff. 
 Qed. 
 
-
-(*evaluation will succeed iff the assignment list binds every variable *)
-Lemma evalCnf_iff_bound (a :assgn) (c : cnf) : (exists v, evalCnf a c = Some v) <-> (exists n, varBound_cnf n c /\ |a| >= n).
+Lemma varsOfCnf_correct N v : v el varsOfCnf N <-> exists C, C el N /\ v el varsOfClause C. 
 Proof. 
-  split; eauto using evalCnf_varBound. 
-  intros (n & H1 & H2). now apply evalCnf_correct with (n:= n). 
+  unfold varsOfCnf. now rewrite in_concat_map_iff. 
+Qed.
+
+Definition assignment_small N a := a <<= varsOfCnf N /\ dupfree a.
+
+Lemma varsOfLiteral_size (l : literal) : size (enc (varsOfLiteral l)) <= size (enc l) + c__listsizeCons + c__listsizeNil. 
+Proof. 
+  unfold varsOfLiteral. destruct l; cbn. rewrite size_list, size_prod. cbn. lia. 
 Qed. 
 
-(*A computable notion of boundedness *)
-Definition clause_maxVar (c : clause) := fold_right (fun '(_, v) acc => Nat.max acc v) 0 c. 
-Definition cnf_maxVar (c : cnf) := fold_right (fun cl acc => Nat.max acc (clause_maxVar cl)) 0 c.
+Lemma varsOfClause_size C : size (enc (varsOfClause C)) <= size (enc C) + (|C|) * (c__listsizeCons + c__listsizeNil). 
+Proof. 
+  unfold varsOfClause. rewrite list_size_concat. 
+  induction C; cbn -[Nat.add]; [easy | ].
+  rewrite !list_size_cons, IHC. 
+  rewrite varsOfLiteral_size. lia.
+Qed. 
 
-Lemma clause_maxVar_bound (c : clause) : varBound_clause (S (clause_maxVar c)) c.
+Lemma varsOfCnf_size N: size (enc (varsOfCnf N)) <= size (enc N) * (1 +( c__listsizeCons + c__listsizeNil)).
+Proof. 
+  unfold varsOfCnf. rewrite list_size_concat. 
+  induction N; cbn -[Nat.add]; [rewrite !size_list; cbn -[Nat.add]; nia | ].
+  rewrite !list_size_cons, IHN. 
+  rewrite varsOfClause_size. 
+  rewrite list_size_length. nia.
+Qed. 
+
+Lemma list_dupfree_incl_length (X : eqType) (a b : list X) : a <<= b -> dupfree a -> |a| <= |b|. 
+Proof. 
+  intros H1 H2. eapply NoDup_incl_length. 
+  - apply dupfree_Nodup, H2.
+  - apply H1. 
+Qed. 
+
+Lemma rem_app_eq (X : eqType) (l1 l2 : list X) (x : X) : rem (l1 ++ l2) x = rem l1 x ++ rem l2 x. 
+Proof. 
+  induction l1; cbn; [easy | ].
+  destruct Dec; cbn. 
+  - fold (rem (l1 ++ l2) x). rewrite IHl1. easy.
+  - fold (rem (l1 ++ l2) x). now rewrite IHl1. 
+Qed. 
+
+Lemma list_rem_size_le (X : eqType) `{H : registered X} (l : list X) x : size (enc (rem l x)) <= size (enc l). 
+Proof. 
+  induction l. 
+  - cbn. lia. 
+  - cbn. destruct Dec; cbn; rewrite !list_size_cons, IHl; lia. 
+Qed. 
+
+Lemma list_incl_dupfree_size (X : eqType) `{registered X} (a b : list X) : a <<= b -> dupfree a -> size (enc a) <= size (enc b). 
+Proof. 
+  intros H1 H2.  revert b H1.
+  induction H2 as [ | a0 a H1 H2 IH]; intros. 
+  - cbn. rewrite !size_list. cbn. lia.
+  - specialize (IH (rem b a0)). 
+    rewrite list_size_cons.
+    cbn. rewrite IH. 
+    2: { 
+      assert (rem (a0 :: a) a0 = a).  
+      { cbn. destruct Dec; [congruence | ]. cbn. 
+       fold (rem a a0). now rewrite rem_id. 
+      } 
+      rewrite <- H3. now apply rem_mono. 
+    } 
+    specialize (H0 a0 (or_introl eq_refl)). apply In_explicit in H0 as (b1 & b2 & ->).
+    rewrite !size_list, !rem_app_eq, !map_app, !sumn_app. cbn. 
+    destruct Dec; cbn; [congruence | ]. 
+    pose (elem_size := fun (x : X) => size (enc x) + c__listsizeCons). 
+    fold elem_size.
+    enough (sumn (map elem_size (rem b1 a0)) <= sumn (map elem_size b1) /\ sumn (map elem_size (rem b2 a0)) <= sumn (map elem_size b2)) as H0.
+    { destruct H0 as [-> ->]. nia. }
+    specialize (list_rem_size_le b1 a0) as F1. 
+    specialize (list_rem_size_le b2 a0) as F2. 
+    rewrite !size_list in F1. rewrite !size_list in F2. 
+    fold elem_size in F1. fold elem_size in F2.
+    split; nia. 
+Qed. 
+
+Lemma assignment_small_size N a : assignment_small N a -> size (enc a) <= size (enc N) * (1 + c__listsizeCons + c__listsizeNil). 
+Proof. 
+  intros [H1 H2].
+  enough (size (enc a) <= size (enc (varsOfCnf N))) as H.
+  { rewrite H. apply varsOfCnf_size. }
+  now eapply list_incl_dupfree_size.
+Qed. 
+
+Definition sat_verifier N (a : assgn) :=
+  evalCnf a N = true /\ assignment_small N a. 
+
+(*we need to show that, given a satisfying assignment for a CNF, we can obtain a small assignment that still satisfies the CNF*)
+Section fixX. 
+  Variable (X : Type).
+  Variable (eqbX : X -> X -> bool). 
+  Context (H : forall x y, x = y <-> eqbX x y = true).
+
+  Fixpoint intersect (a b : list X) := match a with
+  | [] => []
+  | (x::a) => if list_in_decb eqbX b x then x :: intersect a b else intersect a b 
+  end. 
+
+  Lemma in_intersect_iff (a b : list X) : forall x, x el intersect a b <-> x el a /\ x el b. 
+  Proof. 
+    intros x. induction a; cbn; [tauto | ].
+    destruct list_in_decb eqn:H1. 
+    - apply list_in_decb_iff in H1; [ | apply H]. 
+      split; [intros [-> | H2]; firstorder | intros ([-> | H2] & H3); [ easy| right; apply IHa; auto]]. 
+    - apply list_in_decb_iff' in H1; [ | apply H]. 
+      rewrite IHa. split; [ firstorder | intros [[-> | H2] H3]; [congruence | auto]]. 
+  Qed. 
+
+  Fixpoint dedup (a : list X) := match a with 
+  | [] => []
+  | x :: a => if list_in_decb eqbX a x then dedup a else x :: dedup a
+  end. 
+
+  Lemma in_dedup_iff (a : list X) : forall x, x el dedup a <-> x el a. 
+  Proof. 
+    intros x. induction a; cbn; [easy | ]. 
+    destruct list_in_decb eqn:H1. 
+    - apply list_in_decb_iff in H1; [ | apply H]. 
+      rewrite IHa. split; [ easy | intros [-> | H2]; easy].  
+    - apply list_in_decb_iff' in H1; [ | apply H]. 
+      split.
+      + intros [-> | H2]; [easy | right; easy]. 
+      + intros [-> | H2]; [now left | right; easy]. 
+  Qed. 
+
+  Hint Constructors dupfree. 
+  Lemma dupfree_dedup (a : list X) : dupfree (dedup a). 
+  Proof. 
+    induction a; cbn; [ eauto| ]. 
+    destruct list_in_decb eqn:H1. 
+    - apply list_in_decb_iff in H1; easy. 
+    - apply list_in_decb_iff' in H1; [ | easy]. constructor. 
+      + intros H2; apply H1, in_dedup_iff, H2.  
+      + apply IHa. 
+  Qed. 
+End fixX. 
+
+Definition compressAssignment a N := dedup Nat.eqb (intersect Nat.eqb a (varsOfCnf N)). 
+
+Lemma compressAssignment_small a N: assignment_small N (compressAssignment a N).
+Proof. 
+  unfold assignment_small, compressAssignment. split; [ | apply dupfree_dedup; symmetry; apply Nat.eqb_eq].
+  intros x H%in_dedup_iff; [ | symmetry; apply Nat.eqb_eq]. 
+  apply in_intersect_iff in H; [ | symmetry; apply Nat.eqb_eq]. 
+  apply H.  
+Qed. 
+
+Lemma compressAssignment_var_eq a N v : v el varsOfCnf N -> evalVar a v = evalVar (compressAssignment a N) v. 
+Proof. 
+  intros H. unfold compressAssignment. 
+  unfold evalVar. destruct list_in_decb eqn:H1. 
+  - symmetry. rewrite list_in_decb_iff by (symmetry; apply Nat.eqb_eq).
+    apply in_dedup_iff; [ symmetry; apply Nat.eqb_eq | ]. 
+    apply in_intersect_iff; [ symmetry; apply Nat.eqb_eq | ]. 
+    apply list_in_decb_iff in H1; [ | symmetry; apply Nat.eqb_eq]. 
+    easy.
+  - symmetry. 
+    rewrite list_in_decb_iff' by (symmetry; apply Nat.eqb_eq). 
+    intros H2%in_dedup_iff; [ | symmetry; apply Nat.eqb_eq]. 
+    apply in_intersect_iff in H2 as (H2 & _); [ | symmetry; apply Nat.eqb_eq]. 
+    apply list_in_decb_iff' in H1; [ easy | symmetry; apply Nat.eqb_eq]. 
+Qed. 
+
+Lemma compressAssignment_cnf_equiv a N : evalCnf a N = true <-> evalCnf (compressAssignment a N) N = true. 
+Proof. 
+  rewrite !evalCnf_clause_iff. repeat setoid_rewrite evalClause_literal_iff. 
+  split. 
+  - intros H cl H1. specialize (H cl H1) as (l & H & H2). 
+    exists l; split; [apply H | ]. 
+    destruct l. rewrite evalLiteral_var_iff in *. 
+    erewrite <- compressAssignment_var_eq; [ apply H2 | ]. 
+    apply varsOfCnf_correct. exists cl; split; [easy | ].  
+    apply varsOfClause_correct. exists (b, n); split; [easy | ]. 
+    apply varsOfLiteral_correct. exists b; easy.
+  - intros H cl H1. specialize (H cl H1) as (l & H & H2).
+    exists l; split; [apply H | ]. 
+    destruct l. rewrite evalLiteral_var_iff in *. 
+    erewrite compressAssignment_var_eq; [ apply H2 | ]. 
+    apply varsOfCnf_correct. exists cl; split; [easy | ]. 
+    apply varsOfClause_correct. exists (b, n); split; [easy | ]. 
+    apply varsOfLiteral_correct. exists b; easy.
+Qed. 
+
+(*now that we've got the tools to verify the verifier, let's build a boolean verifier and prove its correctness*)
+Definition assignment_small_decb N a := list_incl_decb Nat.eqb a (varsOfCnf N) && dupfreeb Nat.eqb a. 
+Definition sat_verifierb (input : cnf * assgn) :=
+  let (N, a) := input in assignment_small_decb N a && evalCnf a N.
+
+Lemma assignment_small_decb_iff N a : assignment_small_decb N a = true <-> assignment_small N a. 
+Proof. 
+  unfold assignment_small_decb, assignment_small. 
+  rewrite andb_true_iff. 
+  rewrite list_incl_decb_iff; [ | symmetry; apply Nat.eqb_eq]. 
+  rewrite dupfreeb_iff; [ | symmetry; apply Nat.eqb_eq]. 
+  easy.
+Qed. 
+
+Lemma sat_verifierb_correct N a : sat_verifier N a <-> sat_verifierb (N, a) = true.
+Proof. 
+  unfold sat_verifier, sat_verifierb. rewrite and_comm. 
+  rewrite andb_true_iff. rewrite assignment_small_decb_iff. 
+  tauto. 
+Qed. 
+
+(** A computable notion of boundedness *)
+Definition clause_maxVar C := fold_right (fun '(_, v) acc => Nat.max acc v) 0 C. 
+Definition cnf_maxVar N := fold_right (fun C acc => Nat.max acc (clause_maxVar C)) 0 N.
+
+Lemma cnf_maxVar_app N1 N2 : cnf_maxVar (N1 ++ N2) = Nat.max (cnf_maxVar N1) (cnf_maxVar N2). 
+Proof. 
+  induction N1. 
+  - easy.
+  - cbn. fold (cnf_maxVar (N1 ++ N2)). fold (cnf_maxVar N1). rewrite IHN1. lia. 
+Qed. 
+
+Lemma clause_maxVar_bound C : varBound_clause (S (clause_maxVar C)) C.
 Proof.
-  induction c.
+  induction C.
   - cbn. constructor.
   - destruct a. constructor; cbn.
     + lia.   
     + eapply varBound_clause_monotonic.
-      2: apply IHc. unfold clause_maxVar. cbn. lia. 
+      2: apply IHC. unfold clause_maxVar. cbn. lia. 
 Qed.
 
-Lemma cnf_maxVar_bound (c : cnf) : varBound_cnf (S (cnf_maxVar c)) c.
+Lemma cnf_maxVar_bound N : varBound_cnf (S (cnf_maxVar N)) N.
 Proof.
-  induction c.
+  induction N.
   - cbn; constructor.
   - constructor.
     + cbn. eapply varBound_clause_monotonic. 2: apply clause_maxVar_bound. lia. 
-    + eapply varBound_cnf_monotonic. 2: apply IHc. cbn. unfold cnf_maxVar. lia.  
+    + eapply varBound_cnf_monotonic. 2: apply IHN. cbn. unfold cnf_maxVar. lia.  
 Qed. 
 
-(*more helpful properties *)
-(*a characterisation of one processing step of evalClause *)
-Lemma evalClause_step_inv (a : assgn) (cl : clause) (l : literal) (b :bool) : evalClause a (l::cl) = Some b <-> exists b1 b2, evalClause a cl = Some b1 /\ evalLiteral a l = Some b2 /\ b = b1 || b2.
-Proof.
-  induction cl. 
-  - cbn. destruct (evalLiteral a l) eqn:H1.
-    + split. intros H. exists false, b0. split; try split; cbn; try tauto. congruence.
-      intros (b1 & b2 & H2 & H3 & H4). destruct b1; try congruence; cbn in H4; now rewrite <- H4 in H3.
-    + firstorder; congruence. 
- - split.
-   + intros H1. change (match evalClause a (a0::cl) with Some acc => match evalLiteral a l with Some v => Some (acc || v) | None => None end | None => None end = Some b) in H1. 
-     destruct (evalClause a (a0::cl)); try congruence. 
-     destruct (evalLiteral a l); try congruence. 
-     exists b0, b1. split; try split; try tauto. congruence. 
-   + intros (b1 & b2 & H1 & H2 & H3).  
-     change (match evalClause a (a0::cl) with Some acc => match evalLiteral a l with Some v => Some (acc || v) | None => None end | None => None end = Some b). 
-     rewrite H1, H2. now rewrite H3. 
-Qed. 
-
-Lemma evalCnf_step_inv (a : assgn) (cn : cnf) (cl : clause) (b:bool) : evalCnf a (cl::cn) = Some b <-> exists b1 b2, evalCnf a cn = Some b1 /\ evalClause a cl = Some b2 /\ b = b1 && b2.
-Proof.
-  induction cn. 
-  - cbn. destruct evalClause.
-    + split. intros H. exists true, b0. firstorder; try congruence. inv H. eauto.
-      intros (b1 & b2 & H1 & H2 & H3). inv H1; now inv H2. 
-    + firstorder; congruence.  
-  - split.
-    + intros H1. change (match evalCnf a (a0::cn) with Some acc => match evalClause a cl with Some v => Some (acc && v) | None => None end | None => None end = Some b) in H1. 
-      destruct (evalCnf a (a0::cn)); try congruence. 
-      destruct (evalClause a cl); try congruence. 
-      exists b0, b1. split; try split; try tauto. congruence. 
-    + intros (b1 & b2 & H1 & H2 & H3).
-      change (match evalCnf a (a0::cn) with Some acc => match evalClause a cl with Some v => Some (acc && v) | None => None end | None => None end = Some b).
-      rewrite H1, H2. now rewrite H3. 
-Qed. 
-
-Lemma evalClause_literal_iff (a : assgn) (cl : clause) : evalClause a cl = Some true <-> ((exists l, l el cl /\ evalLiteral a l = Some true) /\ varBound_clause (|a|) cl). 
-Proof.
-  induction cl.
-  - cbn. firstorder. congruence. 
-  - split.
-    + intros H. split. 2: now apply evalClause_varBound.
-      apply evalClause_step_inv in H. destruct H as (b1 & b2 & H1 & H2 & H3). destruct b2.
-      * exists a0. firstorder. 
-      * destruct b1. 2: discriminate H3. apply IHcl in H1. destruct H1 as [[l [F1 F2]] _]. exists l. split; [now right | assumption]. 
-    + intros [(l & H1 & H2) H]. destruct H1.
-      * rewrite H0 in *. cbn; rewrite H2. destruct fold_rightOption eqn:H3.
-        -- now rewrite orb_true_r. 
-        -- inv H. apply evalClause_correct with (a:=a) in H6. destruct H6; unfold evalClause in H; congruence.  
-           lia. 
-      * cbn. destruct fold_rightOption eqn:H3. 
-        -- destruct (evalLiteral a a0) eqn:eq.
-           2: {inv H. apply evalLiteral_correct with (a:=a) (b:= b0) (k :=k) in H5. destruct H5; congruence. lia. }
-           destruct b; [reflexivity | ].
-           enough ((exists l, l el cl /\ evalLiteral a l = Some true) /\ varBound_clause (|a|) cl).
-           { apply IHcl in H1. unfold evalClause in H1. congruence. }
-           split; [exists l; firstorder | now inv H]. 
-        -- inv H. apply evalClause_correct with (a:=a) in H6; [| lia].
-           destruct H6 as [v H6]; unfold evalClause in H6; congruence.
-Qed. 
-
-Lemma evalCnf_clause_iff (a : assgn) (cn : cnf) : evalCnf a cn = Some true <-> (forall cl, cl el cn -> evalClause a cl = Some true).
-Proof.
-  induction cn.
-  - cbn. firstorder. 
-  - split.
-    + intros H cl [-> | H1]; apply evalCnf_step_inv in H; destruct H as (b1 & b2 & F1 & F2 & F3); simp_bool'.
-      rewrite IHcn in F1. now apply F1. 
-    + intros H. cbn. destruct (evalClause a a0) eqn:eq. destruct b.
-      1: { assert (evalCnf a cn = Some true) by (apply IHcn; firstorder). unfold evalCnf in H0; now rewrite H0. }
-      all: now specialize (H a0 (or_introl eq_refl)).
-Qed. 
-
-Definition SAT (c : cnf) : Prop := exists (a : assgn), evalCnf a c = Some true. 
-
-(*a verifier for SAT. The condition |a| <= S(cnf_maxVar cn) is needed in order to make sure that it rejects certificates that are too long*)
-Definition sat_verifier (cn : cnf) (a : assgn) :=
-  evalCnf a cn = Some true /\ |a| <= S(cnf_maxVar cn).
-
-(*tools needed for the verification of the verifier*)
-(*now the wanted results: we can shorten the assignment if this doesn't yield to variables being unbound*)
-Lemma bounded_cap_assgn_literal (n : nat) (sgn : bool) (k : nat) : n < k ->
-  forall (a : assgn) (v : bool), evalLiteral a (sgn, n) = Some v -> evalLiteral (takeN a k) (sgn, n) = Some v.
-Proof.
-  intros H a v H1.
-  unfold evalLiteral in *. destruct (nth_error a n) eqn:H2.
-  + specialize (@ntherror_take (bool) a n k b H H2) as H3. now rewrite H3. 
-  + congruence. 
-Qed. 
-
-Lemma bounded_cap_assgn_clause (c : clause) (n : nat) : varBound_clause n c -> forall (a : assgn) (v : bool),
-      evalClause a c = Some v -> evalClause (takeN a n) c  = Some v. 
-Proof.
-  induction c. 
-  - intros H a v. cbn; now destruct v. 
-  - intros H assg v H1. inv H. cbn [evalClause fold_rightOption] in *.
-    destruct (evalLiteral assg (b, k)) eqn:H5. 
-    + rewrite bounded_cap_assgn_literal with (v := b0). 2-3: assumption.
-      destruct (fold_rightOption) eqn:H6 in H1. 
-      -- unfold evalClause in IHc. rewrite IHc with (v:= b1); assumption. 
-      -- congruence. 
-    + exfalso. now destruct fold_rightOption in H1. 
-Qed. 
-
-Lemma bounded_cap_assgn_cnf (c : cnf) (n: nat) : varBound_cnf n c -> forall (a : assgn) (v : bool),
-      evalCnf a c = Some v -> evalCnf (takeN a n) c = Some v.
-Proof.
-  induction c.
-  - intros H a v. cbn; now destruct v. 
-  - intros H assg v H1. inv H. cbn [evalCnf fold_rightOption] in *.
-    destruct (evalClause assg a) eqn:H5.
-    + rewrite bounded_cap_assgn_clause with (v := b). 2-3: assumption.
-      destruct (fold_rightOption) eqn:H6 in H1. 
-      -- unfold evalCnf in IHc. rewrite IHc with (v := b0); assumption. 
-      -- congruence. 
-    + exfalso. now destruct fold_rightOption in H1.
-Qed. 
-
-(*now that we've got the tools to verify the verifier, let's build a boolean verifier and prove its correctness*)
-Definition sat_verifierb (input : cnf * assgn) :=
-  let (cn, a) := input in
-    if leb (|a|) (S(cnf_maxVar cn)) then
-      match evalCnf a cn with Some b => b | None => false end
-    else false.
-
-Lemma sat_verifierb_correct (c : cnf) (a : assgn) : reflect (sat_verifier c a) (sat_verifierb (c, a)).
+(** In principle, we would expect a strict inequality here. The reason for non-strictness is that cnf_maxVar returns 0 in case of an empty CNF. *)
+Lemma clause_maxVar_bound_le C n : varBound_clause n C -> clause_maxVar C <= n.
 Proof. 
-  destruct (sat_verifierb (c, a)) eqn:H; constructor. 
-  - unfold sat_verifierb in H. unfold sat_verifier. destruct (leb (|a|) (S (cnf_maxVar c))) eqn:H1.
-    destruct (evalCnf a c) eqn:H2. split; try congruence; dec_bool. all: congruence. 
-  - intros [H1 H2]. cbn in H. apply leb_correct in H2. rewrite H2, H1 in H. congruence. 
+  induction 1 as [ | ? ? ? ? ? IH]; cbn; [lia | ].
+  rewrite IH. lia. 
 Qed. 
 
-Global Instance term_bool_eqb : computableTime' Bool.eqb (fun _ _ => (1, fun _ _ => (7, tt))). 
+Lemma cnf_maxVar_bound_le N n : varBound_cnf n N -> cnf_maxVar N <= n. 
+Proof. 
+  induction 1 as [ | ? ? ? ? IH]; cbn; [ lia | ].
+  rewrite IH. rewrite clause_maxVar_bound_le by apply H. lia. 
+Qed. 
+
+(** ** extraction *)
+
+(** size of encoding in terms of size of the cnf  *)
+Definition c__clauseSize1 := c__listsizeCons + c__sizeBool + c__natsizeO + 4 + c__listsizeNil.
+Lemma clause_enc_size_bound (c : clause) : size (enc c) <= c__natsizeS * (clause_maxVar c + 1) * (size_clause c + 1) + c__clauseSize1 * (size_clause c + 1). 
+Proof. 
+  induction c.
+  - rewrite size_list; cbn -[Nat.mul Nat.add]. unfold c__clauseSize1. lia. 
+  - rewrite list_size_cons. rewrite IHc. cbn -[Nat.mul Nat.add]. destruct a. 
+    fold (clause_maxVar c). 
+    rewrite size_prod; cbn -[Nat.mul Nat.add]. rewrite size_bool. rewrite size_nat_enc. 
+    unfold size_clause. 
+    unfold c__clauseSize1. nia. 
+Qed. 
+
+Definition c__cnfSize1 := c__listsizeNil + c__listsizeCons + c__clauseSize1.
+Lemma cnf_enc_size_bound (c : cnf) : size (enc c) <= c__natsizeS * (cnf_maxVar c + 1) * (size_cnf c + 1) + (size_cnf c + 1) * c__cnfSize1.
+Proof. 
+  induction c. 
+  - rewrite size_list. cbn -[Nat.mul Nat.add]. unfold c__cnfSize1. nia.
+  - rewrite list_size_cons. rewrite clause_enc_size_bound. 
+    cbn -[c__clauseSize1 c__cnfSize1 c__listsizeCons c__natsizeS].
+    fold (cnf_maxVar c). 
+    replace (size_clause a + sumn (map size_clause c) + S (|c|) + 1) with (size_clause a + size_cnf c + 2) by (unfold size_cnf; cbn; lia).
+    rewrite IHc. 
+    (*nia and leq_crossout need some help to see that this holds*)
+    replace_le (c__natsizeS * (clause_maxVar a + 1) * (size_clause a + 1) + c__clauseSize1 * (size_clause a + 1) + (c__natsizeS * (cnf_maxVar c + 1) * (size_cnf c + 1) + (size_cnf c + 1) * c__cnfSize1) + c__listsizeCons) 
+    with (c__natsizeS * (Nat.max (cnf_maxVar c) (clause_maxVar a) + 1) * (size_clause a + size_cnf c + 2) + c__clauseSize1 * (size_clause a + 1) + (size_cnf c + 1) * c__cnfSize1 + c__listsizeCons) by nia. 
+    unfold c__cnfSize1. nia.
+Qed. 
+
+(** conversely, we can bound the size of the cnf in terms of the encoding size *)
+(** we only get a quadratic bound because of the huge overapproximation by taking cnf_maxVar *)
+
+Lemma clause_maxVar_size_enc_bound (c : clause) : clause_maxVar c + 1 <= size (enc c).
+Proof. 
+  induction c; cbn; [rewrite size_list; unfold c__listsizeNil; lia| ]. 
+  fold (clause_maxVar c). destruct a. rewrite list_size_cons, size_prod. cbn. 
+  rewrite size_nat_enc_r with (n := n) at 1. nia. 
+Qed. 
+
+Lemma clause_size_enc_bound (c : clause) : size_clause c + 1 <= size (enc c). 
+Proof. 
+  unfold size_clause. induction c. 
+  - rewrite size_list; cbn; unfold c__listsizeNil; lia. 
+  - rewrite list_size_cons; cbn. unfold c__listsizeCons; lia. 
+Qed. 
+
+
+Lemma clause_size_total_enc_bound (c : clause) : (size_clause c + 1) * (clause_maxVar c + 1) <= size (enc c) * size (enc c). 
+Proof. 
+  now rewrite clause_maxVar_size_enc_bound, clause_size_enc_bound. 
+Qed. 
+
+Lemma cnf_size_enc_bound (c : cnf) : (size_cnf c + 1) <= size (enc c). 
+Proof. 
+  induction c; cbn. 
+  - rewrite size_list; unfold c__listsizeNil; lia. 
+  - replace (size_clause a + sumn (map size_clause c) + S (|c|) + 1) with ((size_clause a + 1) + (size_cnf c + 1)). 
+    2: { unfold size_cnf. lia. }
+    rewrite IHc. rewrite list_size_cons. rewrite clause_size_enc_bound. lia.
+Qed. 
+
+Lemma cnf_maxVar_size_enc_bound (c : cnf) : cnf_maxVar c + 1 <= size (enc c). 
+Proof. 
+  induction c; cbn. 
+  - rewrite size_list; unfold c__listsizeNil; lia.
+  - fold (cnf_maxVar c). rewrite list_size_cons. 
+    specialize (clause_maxVar_size_enc_bound a). unfold c__listsizeCons. lia. 
+Qed. 
+
+Lemma cnf_size_total_enc_bound (c : cnf) : (size_cnf c + 1) * (cnf_maxVar c + 1) <= size (enc c) * size (enc c). 
+Proof. 
+  rewrite cnf_maxVar_size_enc_bound, cnf_size_enc_bound.  lia. 
+Qed. 
+
+
+(** extraction of evalVar *)
+Definition c__evalVar := 7. 
+Definition evalVar_time a (v : var) := list_in_decb_time (fun x y => c__nat_eqb2 + nat_eqb_time x y) a v + c__evalVar.
+Instance term_evalVar : computableTime' evalVar (fun a _ => (1, fun v _ => (evalVar_time a v, tt))). 
+Proof. 
+  extract. solverec. unfold evalVar_time, c__evalVar; solverec. 
+Defined. 
+
+Definition c__evalVarBound := c__nat_eqb2 + c__list_in_decb. 
+Definition poly__evalVar n := (n + 1) * (c__evalVarBound + (n + size(enc tt)+ 1) * c__nat_eqb) + c__evalVar.
+Lemma evalVar_time_bound a v : evalVar_time a v <= poly__evalVar (size (enc a) + size (enc v)). 
+Proof. 
+  unfold evalVar_time. 
+  change (fun x y => c__nat_eqb2 + nat_eqb_time x y) with ((fun z x y => c__nat_eqb2 + nat_eqb_time x y) tt). 
+  rewrite list_in_decb_time_bound_env. 
+  2: { 
+    split. 
+    - intros. rewrite nat_eqb_time_bound_l. replace_le (size (enc a0)) with (size (enc a0) + size (enc b) + size (enc y)) by nia at 1. instantiate (2 := fun n => c__nat_eqb2 + (n + 1) * c__nat_eqb).
+      cbn -[Nat.add]. instantiate (1 := registered_unit_enc). nia. 
+    - smpl_inO. 
+  } 
+  rewrite list_size_length. unfold poly__evalVar, c__evalVarBound. nia. 
+Qed. 
+
+Lemma evalVar_poly : monotonic poly__evalVar /\ inOPoly poly__evalVar. 
+Proof. 
+  split; unfold poly__evalVar; smpl_inO. 
+Qed. 
+
+
+Definition c__eqbBool := 7.
+Instance term_bool_eqb : computableTime' Bool.eqb (fun _ _ => (1, fun _ _ => (c__eqbBool, tt))). 
 Proof.
-  extract.
+  extract. unfold c__eqbBool.
   solverec. 
 Qed.
 
-Definition evalLiteral_time (a : assgn) (l : literal) := match l with (_, v) => callTime2 (@nth_error_time bool) a v + 18 end. 
-
+(*evalLiteral*)
+Definition c__evalLiteral := c__eqbBool + 7. 
+Definition evalLiteral_time a (l : literal) := match l with (_, v) => evalVar_time a v + c__evalLiteral end. 
 Instance term_evalLiteral : computableTime' evalLiteral (fun a _ => (1, fun l _ => (evalLiteral_time a l, tt))). 
 Proof. 
-  extract. 
-  solverec. 
+  extract. solverec. unfold c__evalLiteral. solverec. 
 Qed. 
 
-Section fixXY.
-  Variable (X Y : Type).
-  Context {H : registered X}.
-  Context {H0 : registered Y}. 
-  Fixpoint fold_rightOption_time (f : Y -> X -> option X) (tf : timeComplexity (Y -> X -> option X)) (l : list Y) (acc : option X) :=
-    match l with [] => 4
-               | l::ls => (match fold_rightOption f acc ls with Some acc' => callTime2 tf l acc'
-                                                       | None => 0 end)
-                   + 15 + fold_rightOption_time f tf ls acc
- end. 
-
-  Global Instance term_fold_rightOption:  computableTime' (@fold_rightOption X Y) (fun f t__f => (1, fun acc _ => (5, fun l _ => (fold_rightOption_time f t__f l acc, tt)))). 
-  Proof.
-    extract. 
-    solverec. 
-    - unfold fold_rightOption in H3. assert (x4 = x5) by congruence. now rewrite H5. 
-    - unfold fold_rightOption in H3; congruence. 
-  Qed. 
-
-End fixXY. 
-
-(*we need to factor out the fold step function first and extract it separately *)
-Definition evalClause_step (a : assgn):=
-  fun (lit : literal) (acc : bool)  => match evalLiteral a lit with
-                                  | Some v => Some (acc || v)
-                                  | None => None
-                                 end. 
-
-Instance term_evalClause_step : computableTime' evalClause_step (fun a _ => (1, fun lit _ => (1, fun acc _ => (evalLiteral_time a lit + 12, tt)))). 
+Definition c__evalLiteralBound := 1. 
+Definition poly__evalLiteral n := poly__evalVar n + c__evalLiteral.
+Lemma evalLiteral_time_bound a l : evalLiteral_time a l <= poly__evalLiteral (size (enc a) + size (enc l)). 
 Proof. 
-  extract. 
-  solverec.
+  unfold evalLiteral_time. destruct l. rewrite evalVar_time_bound. 
+  poly_mono evalVar_poly. 
+  2: (replace_le (size (enc n)) with (size (enc (b, n))) by (rewrite size_prod; cbn; lia)); reflexivity. 
+  unfold poly__evalLiteral; lia.
+Qed. 
+Lemma evalLiteral_poly : monotonic poly__evalLiteral /\ inOPoly poly__evalLiteral. 
+Proof. 
+  split; unfold poly__evalLiteral; smpl_inO; apply evalVar_poly.
 Qed. 
 
-Definition evalClause_time (a : assgn) (cl : clause):= fold_rightOption_time (evalClause_step a) (fun lit _ => (1, fun acc _ => (evalLiteral_time a lit + 12, tt))) cl (Some false) + 9 . 
 
-Instance term_evalClause : computableTime' evalClause  (fun (a: assgn) (_ : unit) =>
-  (1, fun (cl : clause) (_ : unit) => (evalClause_time a cl, tt))).  
-Proof.
-  assert (H : extEq (fun a l => fold_rightOption (evalClause_step a) (Some false) l) evalClause). 
-  { unfold extEq, evalClause, evalClause_step. auto. }
-  eapply computableTimeExt. apply H. 
-  extract. 
-  solverec. 
+(*evalClause *)
+Definition c__evalClause_step := c__evalLiteral + 7.
+Definition evalClause_step_time a (l : literal) (acc : bool) := match l with (_, v) => evalVar_time a v + c__evalClause_step end. 
+Instance term_evalClause_step : computableTime' evalClause_step (fun a _ => (1, fun l _ => (1, fun acc _ => (evalClause_step_time a l acc, tt)))).
+Proof. 
+  extract. solverec. unfold c__evalClause_step. solverec. 
+Defined.
+
+Definition c__evalClause := c__fold_right + 4.
+Definition evalClause_time a (c : clause) := fold_right_time (evalClause_step a) (fun l acc => 1 + evalClause_step_time a l acc) c false + c__evalClause.
+Instance term_evalClause : computableTime' evalClause (fun a _ => (1, fun c _ => (evalClause_time a c, tt))). 
+Proof. 
+  extract. solverec. unfold evalClause_time, c__evalClause. solverec. 
+Defined. 
+
+Definition c__evalClauseBound := c__evalClause_step + c__fold_right. 
+Definition poly__evalClause n := (n + 1) * (1 + poly__evalVar ((n+1) * c__sizeBool + n) + c__evalClauseBound) + c__evalClause. 
+Lemma evalClause_time_bound a c : evalClause_time a c <= poly__evalClause (size (enc a) + size (enc c)). 
+Proof. 
   unfold evalClause_time. 
-  solverec. 
-Qed. 
-
-
-Definition evalCnf_step (a : assgn) :=
-  fun (cl : clause) (acc : bool) => match evalClause a cl with
-                                | Some v => Some (acc && v)
-                                | None => None
-                              end. 
-
-Instance term_evalCnf_step : computableTime' evalCnf_step (fun a _ => (1, fun cl _ => (1, fun acc _ => (evalClause_time a cl + 16, tt)))).
-Proof.
-  extract. solverec. 
-Qed.
-
-
-Definition evalCnf_time (a : assgn) (cn : cnf) := fold_rightOption_time (evalCnf_step a) (fun cl _ => (1, fun acc _ => (evalClause_time a cl  + 16, tt))) cn (Some true) + 9.
-
-Instance term_evalCnf : computableTime' evalCnf (fun (a : assgn) _ => (1, fun cn _ => (evalCnf_time a cn , tt))). 
-Proof.
-  assert (H : extEq (fun a l => fold_rightOption (evalCnf_step a) (Some true) l) evalCnf). 
-  { unfold extEq, evalCnf, evalCnf_step. auto. }
-  eapply computableTimeExt. apply H. 
-  extract.
-  solverec. 
-  unfold evalCnf_time; solverec. 
-Qed. 
-
-(*extraction of the verifier *)
-
-Require Import Undecidability.L.Datatypes.Lists.
-
-Definition clause_maxVar_step := fun (l : literal) (acc : nat) => let '(_, v) := l in max acc v. 
-Instance term_clause_maxVar_step : computableTime' clause_maxVar_step (fun l _ => (1, fun acc _ => (let '(_, v):= l in 18 + 15 * min acc v, tt))). 
-Proof. extract. solverec. Qed.
-
-Definition clause_maxVar_time (c : clause) := fold_right_time clause_maxVar_step (fun (l : literal) (_ : unit) =>
-     (1, fun (acc : nat) (_ : unit) => (let '(_, v) := l in 18 + 15 * Init.Nat.min acc v, tt))) c 0 + 11. 
-Instance term_clause_maxVar : computableTime' clause_maxVar (fun cl _ => (clause_maxVar_time cl, tt)).  
-Proof.
-  assert (H' : extEq (fun c => fold_right clause_maxVar_step 0 c) clause_maxVar).
-  { intros c. unfold extEq. unfold clause_maxVar.
-    induction c. now cbn.
-    cbn. destruct a. cbn. now rewrite IHc. }
-  apply (computableTimeExt H'). extract. solverec. unfold clause_maxVar_time. solverec.
-Qed. 
-
-Definition cnf_maxVar_step := fun (cl : clause) (acc : nat)  => max acc (clause_maxVar cl). 
-Instance term_cnf_maxVar_step : computableTime' cnf_maxVar_step (fun cl _ => (1, fun acc _ => (clause_maxVar_time cl + 15 * min acc (clause_maxVar cl) + 14, tt))).
-Proof. extract. solverec. Qed. 
-
-Definition cnf_maxVar_time (c : cnf) := fold_right_time cnf_maxVar_step
-    (fun (cl : clause) (_ : unit) =>
-     (1,
-     fun (acc : nat) (_ : unit) =>
-     (clause_maxVar_time cl + 15 * Init.Nat.min acc (clause_maxVar cl) + 14, tt))) c 0 + 11.
-Instance term_cnf_maxVar : computableTime' cnf_maxVar (fun (c : cnf) _  => (cnf_maxVar_time c, tt)). 
-Proof. 
-  assert (H' : extEq (fun c => fold_right cnf_maxVar_step 0 c) cnf_maxVar).
-  { intros c. unfold extEq, cnf_maxVar. induction c. now cbn. 
-    cbn. now rewrite IHc. }
-  apply (computableTimeExt H'). extract; solverec. 
-  unfold cnf_maxVar_time. solverec. 
-Qed. 
-
-
-Definition sat_verifierb_time (c : cnf) (a : assgn) :=   11 * (| a |) + cnf_maxVar_time c + 14 * Init.Nat.min (| a |) (1 + cnf_maxVar c) +  evalCnf_time a c + 39.
-Instance term_sat_verifierb : computableTime' sat_verifierb (fun input _ => (let (c, a) := input in sat_verifierb_time c a, tt)). 
-Proof.
-  extract. solverec; unfold sat_verifierb_time; solverec. 
-Qed. 
-
-(*polynomial time bounds for sat_verifierb and the functions it uses*)
-Proposition max_bound a b : max a b <= a + b.
-Proof. lia. Qed. 
-
-Require Import Undecidability.L.Complexity.PolyBounds.
-
-(* eval bounds*)
-(*first of all: a bound for fold_rightOption; adapted from the fold_right bound *)
-Section fixXYZ_fold_rightOption.
-  Context {X Y Z: Type}.
-  Context {H:registered X}.
-  Context {H0: registered Y}.
-  Context {H1 : registered Z}.
-
-  Lemma fold_rightOption_time_bound_env (step : Z -> Y -> X -> option X) (stepT : Z -> timeComplexity (Y -> X -> option X)) :
-    (exists (f : nat -> nat), (forall (acc : X) (ele : Y) (env : Z), callTime2 (stepT env) ele acc <= f(size(enc acc) + size(enc ele) + size(enc env))) /\ inOPoly f /\ monotonic f)
-    -> (exists (c__out : nat), forall (acc : X) (ele : Y) (env : Z), size(enc (step env ele acc)) <= size(enc acc) + size(enc ele) + size(enc env) + c__out)
-    -> exists (f : nat -> nat), (forall (l : list Y) (acc : option X) (env : Z), fold_rightOption_time (step env) (stepT env) l acc <= f(size(enc l) + size(enc acc) + size(enc env))) /\ inOPoly f /\ monotonic f.
-  Proof.
-    intros (f__step & H2 & H3 & H4) (c__out & F). 
-    evar (f : nat -> nat). exists f. split.
-    - intros l init env.
-      (* we first show that the output size of foldr on every suffix is polynomial *)
-      assert (forall l' l'', l = l' ++ l'' -> forall v, fold_rightOption (step env) init l'' = Some v -> size(enc v) <= size(enc init) + size(enc l'') + (|l''|) * (size(enc env) + c__out)).
-      {
-        intros l' l''; revert l'. induction l''.
-        + cbn. intros. rewrite H6. rewrite size_option. lia.
-        + intros. cbn in H6. destruct fold_rightOption eqn:H7.
-          * specialize (size_option (Some v)) as H8. cbn in H8. assert (size(enc v) <= size(enc (Some v))) as H9 by lia; rewrite H9, <- H6. clear H8 H9.
-            rewrite F. rewrite IHl''. 3: reflexivity. 2: {now rewrite app_comm_cons' in H5. }
-            rewrite list_size_cons. solverec. 
-          * congruence.
-      }
-
-      instantiate (f := fun n => 4 + n * f__step((S c__out) * n * n + n) + 15 * n). subst f.
-      unfold fold_rightOption_time. 
-      induction l.
-      + solverec.
-      + rewrite IHl.
-        * destruct (fold_rightOption) eqn:H6.
-          -- rewrite H2. unfold monotonic in H4.
-             rewrite H4 with (x' := size(enc init) + size(enc l) + (|l|) * (size(enc env) + c__out) + size(enc a) + size(enc env)).
-             2: {
-               rewrite H5. 3: apply H6. 2: assert (a::l = [a] ++ l) as H7 by reflexivity; apply H7. now lia. 
-             }
-
-             rewrite H4 with (x' := (S c__out) * (size(enc(a::l)) + size(enc init) + size(enc env)) *  (size(enc(a::l)) + size(enc init) + size(enc env)) + (size(enc(a::l)) + size(enc init) + size(enc env))). 
-             2: {clear IHl. rewrite list_size_length. rewrite list_size_cons. cbn; nia. }
-
-             setoid_rewrite H4 with (x' := (S c__out) *( size(enc(a::l)) + size(enc init) + size(enc env)) *  (size(enc(a::l)) + size(enc init) + size(enc env)) + (size(enc(a::l)) + size(enc init) + size(enc env))) at 2. 
-             2: {clear IHl. rewrite list_size_cons. cbn; nia. }
-
-             rewrite list_size_cons at 7. rewrite list_size_cons at 10. solverec. 
-         -- unfold monotonic in H4. rewrite H4 with (x' := (S c__out) *( size(enc(a::l)) + size(enc init) + size(enc env)) *  (size(enc(a::l)) + size(enc init) + size(enc env)) + (size(enc(a::l)) + size(enc init) + size(enc env))). 
-             2: {clear IHl. rewrite list_size_cons. cbn; nia. }
-
-             rewrite list_size_cons at 4. rewrite list_size_cons at 7. solverec. 
-
-       * clear IHl. intros. apply H5 with (l' := a::l'); now firstorder.
-    - subst f; split; smpl_inO. apply inOPoly_comp; smpl_inO. 
-  Qed. 
-End fixXYZ_fold_rightOption.
-
-Lemma evalLiteral_time_bound : exists (f : nat -> nat), (forall (a : assgn) (l : literal), evalLiteral_time a l <= f (size (enc a))) /\ inOPoly f /\ monotonic f.
-Proof.
-  destruct (nth_error_time_bound (X := bool)) as (f & H1 & H2 & H3). 
-  exists (fun n => f n + 18). split.
-  - intros. unfold evalLiteral_time. destruct l. now rewrite H1. 
-  - split; smpl_inO.
-Qed. 
-
-Require Import Undecidability.L.Datatypes.LBool.
-
-Lemma evalClause_time_bound : exists (f : nat -> nat), (forall (a : assgn) (cl : clause), evalClause_time a cl <= f (size (enc a) + size(enc cl)) ) /\ inOPoly f /\ monotonic f.
-Proof.
-  pose (stepT := fun a => fun (lit : literal) (_ : unit) => (1, fun (_ : bool) (_ : unit) => (evalLiteral_time a lit + 12, tt))).
-
-  assert (exists (f : nat -> nat), (forall (acc : bool) (lit : literal) (a : assgn), callTime2 (stepT a) lit acc <= f(size(enc acc) + size(enc lit) + size(enc a))) /\ inOPoly f /\ monotonic f). 
-  {
-    destruct (evalLiteral_time_bound) as (f' & H1 & H2 & H3).
-    evar (f : nat -> nat). exists f. split.
-    - intros. cbn. rewrite H1.
-      unfold monotonic in H3. rewrite H3 with (x' := (size(enc acc) + size(enc lit) + size(enc a))) by lia. 
-      instantiate (f := fun n => f' n + 13). subst f. lia. 
-    - subst f; split; smpl_inO. 
+  change (fun l acc => 1 + evalClause_step_time a l acc) with ((fun a l acc => 1 + evalClause_step_time a l acc) a). 
+  rewrite fold_right_time_bound_env. 
+  3: { 
+    split; [intros| ]. 
+    - rewrite size_bool. instantiate (1 := fun n => c__sizeBool). nia.
+    - smpl_inO. 
   }
-
-  assert (exists c__out, forall (acc : bool) (lit : literal) (a : assgn), size(enc (evalClause_step a lit acc)) <= size(enc acc) + size(enc lit) + size(enc a) + c__out).
-  {
-    exists 9. intros. unfold evalClause_step. destruct (evalLiteral); rewrite size_option. repeat rewrite size_bool. all: lia. 
-  }
-
-  destruct (fold_rightOption_time_bound_env H H0) as (f & H1 & H2 & H3). 
-  exists (fun n => f (n + 9) + 9). split.
-  - unfold evalClause_time. intros a cl. fold (stepT a). rewrite H1. unfold monotonic in H3.
-    rewrite H3 with (x' := size(enc a) + size(enc cl) + 9). lia. 
-    rewrite size_option, size_bool. lia. 
-  - split; smpl_inO. apply inOPoly_comp; smpl_inO. 
-Qed. 
-
-Lemma evalCnf_time_bound : exists (f : nat -> nat), (forall (a : assgn) (c : cnf), evalCnf_time a c <= f(size(enc a) + size(enc c))) /\ inOPoly f /\ monotonic f.
-Proof.
-  pose (stepT := fun a => fun (cl : clause) (_ : unit) => (1, fun (acc : bool) (_ : unit) => (evalClause_time a cl + 16, tt))).
-  assert (exists (f : nat -> nat), (forall (acc : bool) (cl : clause) (a : assgn), callTime2 (stepT a) cl acc <= f(size(enc acc) + size(enc cl) + size(enc a))) /\ inOPoly f /\ monotonic f). 
-  {
-    destruct (evalClause_time_bound) as (f' & H1 & H2 & H3).
-    evar (f : nat -> nat). exists f. split.
-    - intros. cbn. rewrite H1.
-      unfold monotonic in H3. rewrite H3 with (x' := (size(enc acc) + size(enc cl) + size(enc a))) by lia.
-      instantiate (f := fun n => f' n + 17). subst f; lia. 
-    - subst f; split; smpl_inO. 
-  }
-
-  assert (exists c__out, forall (acc : bool) (cl : clause) (a : assgn), size(enc (evalCnf_step a cl acc)) <= size(enc acc) + size(enc cl) + size(enc a) + c__out). 
-  {
-    exists 9. intros. unfold evalCnf_step. destruct evalClause; rewrite size_option.  repeat rewrite size_bool. all: lia. 
-  }
-
-  destruct (fold_rightOption_time_bound_env H H0) as (f & H1 & H2 & H3).
-  exists (fun n => f(n+9) + 9). split. 
-  - unfold evalCnf_time. intros. fold (stepT a). rewrite H1. unfold monotonic in H3.
-    rewrite H3 with (x' := size(enc a) + size(enc c) + 9). lia. 
-    rewrite size_option, size_bool. lia. 
-  - split; smpl_inO. apply inOPoly_comp; smpl_inO. 
-Qed. 
-
-
-(*cnf_maxVar bounds *)
-Lemma clause_maxVar_time_bound : exists (f : nat -> nat), (forall (c : clause), clause_maxVar_time c <= f(size(enc c))) /\ inOPoly f /\ monotonic f. 
-Proof.
-  unfold clause_maxVar_time. 
-  pose (stepT := (fun (l : bool * nat) (_ : unit) =>
-        (1, fun (acc : nat) (_ : unit) => (let '(_, v) := l in 18 + 15 * Init.Nat.min acc v, tt)))).
-  assert (exists (f : nat -> nat), (forall (acc : nat) (l : literal), callTime2 stepT l acc <= f(size (enc acc) + size(enc l))) /\ inOPoly f /\ monotonic f). 
-  {
-    evar (f : nat -> nat). exists f. split.
-    - intros. destruct l. cbn -[Nat.mul Nat.add]. rewrite Nat.le_min_r. rewrite size_prod; cbn [fst snd]. 
-      specialize size_nat_enc_r with (n := n). 
-      instantiate (f := fun n => 19 + 15 * n). subst f; solverec. 
-    - subst f; split; smpl_inO. 
-  }
-  assert (exists c__out c__out', forall (acc : nat) (l : literal), size(enc (clause_maxVar_step l acc)) <= size(enc acc) + c__out' * size(enc l) + c__out). 
-  {
-    exists 0, 1. intros. 
-    unfold clause_maxVar_step. destruct l. rewrite size_prod; cbn [fst snd].
-    repeat rewrite size_nat_enc. rewrite max_bound. lia. 
-  }
-  fold stepT. 
-  specialize (fold_right_time_bound H H0) as (f & H1 & H2 & H3). 
-  exists (fun n => f (n + 4) + 11). split.
-  - intros. specialize (H1 c 0). rewrite H1. rewrite size_nat_enc. solverec. 
-  - split; smpl_inO. apply inOPoly_comp; smpl_inO. 
-Qed.
-
-Lemma cnf_maxVar_time_bound : exists (f : nat -> nat), (forall (c : cnf), cnf_maxVar_time c <= f(size (enc c))) /\ inOPoly f /\ monotonic f. 
-Proof.
-  pose (stepT := (fun (cl : list (bool * nat)) (_ : unit) =>
-   (1,
-   fun (acc : nat) (_ : unit) =>
-     (clause_maxVar_time cl + 15 * Init.Nat.min acc (clause_maxVar cl) + 14, tt)))).
-  unfold cnf_maxVar_time. fold stepT. 
-
-  assert (exists (f : nat -> nat), (forall (acc : nat) (l : clause), callTime2 stepT l acc <= f(size (enc acc) + size(enc l))) /\ inOPoly f /\ monotonic f). 
-  {
-    destruct (clause_maxVar_time_bound) as (f' & H1 & H2 & H3).
-    evar (f : nat -> nat). exists f. split.
-    - intros; cbn -[Nat.add Nat.mul]. rewrite H1. rewrite Nat.le_min_l. 
-      unfold monotonic in H3. rewrite H3 with (x' := size(enc acc) + size(enc l)) by lia.
-      specialize size_nat_enc_r with (n := acc). 
-      instantiate (f := fun n => f' n + 15 * n + 15). subst f. solverec. 
-   - subst f; split; smpl_inO. 
+  2: { 
+    split; [intros | ]. 
+    - unfold evalClause_step_time. destruct ele. rewrite evalVar_time_bound.  
+      instantiate (1 := fun n => 1 + poly__evalVar n + c__evalClause_step). cbn - [Nat.add]. 
+      poly_mono evalVar_poly. 
+      2: { replace_le (size (enc env) + size (enc n)) with (size (enc acc) + size (enc (b, n)) + size (enc env)) by (rewrite size_prod; cbn; lia). reflexivity. }
+      lia. 
+    - smpl_inO. apply evalVar_poly. 
   } 
-  assert (exists c__out c__out', forall (acc : nat) (c : clause), size(enc (cnf_maxVar_step c acc)) <= size(enc acc) + c__out' * size(enc c) + c__out).
-  {
-    exists 0, 1. intros. 
-    unfold cnf_maxVar_step. repeat rewrite size_nat_enc. rewrite max_bound. 
-    enough (clause_maxVar c * 4 <= size(enc c)) by lia.
-    induction c. 
-    - cbn. lia.
-    - cbn. destruct a. rewrite list_size_cons. rewrite max_bound. rewrite size_prod; cbn [fst snd].
-      recRel_prettify2. rewrite Nat.mul_comm. rewrite IHc. rewrite size_nat_enc. solverec. 
+  cbn -[Nat.add]. poly_mono evalVar_poly. 
+  2: { rewrite list_size_length. rewrite size_bool. reflexivity. }
+  rewrite list_size_length.
+  unfold poly__evalClause, c__evalClauseBound. 
+  poly_mono evalVar_poly. 
+  2: { instantiate (1 := (size (enc a) + size (enc c) + 1) * c__sizeBool + (size (enc a) + size (enc c))). nia. }
+  nia.
+Qed. 
+Lemma evalClause_poly : monotonic poly__evalClause /\ inOPoly poly__evalClause. 
+Proof. 
+  split; unfold poly__evalClause; smpl_inO. 
+  - apply evalVar_poly. 
+  - apply inOPoly_comp; [apply evalVar_poly | apply evalVar_poly | smpl_inO]. 
+Qed. 
+
+
+(*evalCnf *)
+Definition c__evalCnf_step := 7.
+Definition evalCnf_step_time a (c : clause) := evalClause_time a c + c__evalCnf_step.
+Instance term_evalCnf_step : computableTime' evalCnf_step (fun a _ => (1, fun c _ => (1, fun acc _ => (evalCnf_step_time a c, tt)))). 
+Proof. 
+  extract. solverec. unfold evalCnf_step_time, c__evalCnf_step. solverec. 
+Defined. 
+
+Definition c__evalCnf := c__fold_right + 4.
+Definition evalCnf_time a (cn : cnf) := fold_right_time (evalCnf_step a) (fun cl _ => 1 + evalCnf_step_time a cl) cn true + c__evalCnf.
+Instance term_evalCnf : computableTime' evalCnf (fun a _ => (1, fun c _ => (evalCnf_time a c, tt))). 
+Proof. 
+  extract. solverec. unfold evalCnf_time, c__evalCnf. solverec. 
+Defined. 
+
+Definition c__evalCnfBound := c__evalCnf_step + c__fold_right. 
+Definition poly__evalCnf n := (n + 1) * (1 + poly__evalClause ((n+1) * c__sizeBool + n) + c__evalCnfBound) + c__evalCnf. 
+Lemma evalCnf_time_bound a c : evalCnf_time a c <= poly__evalCnf (size (enc a) + size (enc c)). 
+Proof. 
+  unfold evalCnf_time. 
+  change (fun cl _ => 1 + evalCnf_step_time a cl) with ((fun a cl (_ : bool) => 1 + evalCnf_step_time a cl ) a). 
+  rewrite fold_right_time_bound_env. 
+  3: { 
+    split; [intros| ]. 
+    - rewrite size_bool. instantiate (1 := fun n => c__sizeBool). nia.
+    - smpl_inO. 
   }
-
-  specialize (fold_right_time_bound H H0) as (f & H1 & H2 & H3). 
-  exists (fun n => f (n + 4) + 11). split.
-  - intros. rewrite H1. rewrite size_nat_enc. solverec. 
-  - split; smpl_inO. apply inOPoly_comp; smpl_inO. 
+  2: { 
+    split; [intros | ]. 
+    - unfold evalCnf_step_time. rewrite evalClause_time_bound.  
+      instantiate (1 := fun n => 1 + poly__evalClause n + c__evalCnf_step). cbn - [Nat.add]. 
+      poly_mono evalClause_poly. 
+      2: { replace_le (size (enc env) + size (enc ele)) with (size (enc acc) + size (enc ele) + size (enc env)) by (lia). reflexivity. }
+      lia. 
+    - smpl_inO. apply evalClause_poly. 
+  } 
+  cbn -[Nat.add]. poly_mono evalClause_poly. 
+  2: { rewrite list_size_length. rewrite size_bool. reflexivity. }
+  rewrite list_size_length.
+  unfold poly__evalCnf, c__evalCnfBound. 
+  poly_mono evalClause_poly. 
+  2: { instantiate (1 := (size (enc a) + size (enc c) + 1) * c__sizeBool + (size (enc a) + size (enc c))). nia. }
+  nia.
+Qed. 
+Lemma evalCnf_poly : monotonic poly__evalCnf /\ inOPoly poly__evalCnf. 
+Proof. 
+  split; unfold poly__evalCnf; smpl_inO. 
+  - apply evalClause_poly. 
+  - apply inOPoly_comp; [apply evalClause_poly | apply evalClause_poly | smpl_inO]. 
 Qed. 
 
-Lemma sat_verifierb_time_bound : exists (f : nat -> nat), (forall (c : cnf) (a : assgn), sat_verifierb_time c a <= f(size(enc c) + size(enc a))) /\ inOPoly f /\ monotonic f. 
-Proof.
-  destruct (evalCnf_time_bound) as (h & H1 & H2 & H3).
-  destruct (cnf_maxVar_time_bound) as (g & F1 & F2 & F3). 
-  evar (f : nat -> nat). exists f; split.
-  - intros. unfold sat_verifierb_time. rewrite F1, H1. rewrite Nat.le_min_l. 
-    rewrite list_size_length.
-    unfold monotonic in F3. rewrite F3 with (x' := size(enc c) + size(enc a)) by lia. 
-    setoid_rewrite Nat.add_comm with (n := size(enc a)) (m := size(enc c)).  
-    instantiate (f := fun n => 25 *n + g n + h n + 39). subst f. solverec. 
-  - subst f; split; smpl_inO. 
+(*varsOfLiteral *)
+Definition c__varsOfLiteral := 7.
+Instance term_varsOfLiteral : computableTime' varsOfLiteral (fun l _ => (c__varsOfLiteral, tt)). 
+Proof. 
+  extract. solverec. unfold c__varsOfLiteral; solverec. 
+Defined. 
+
+(*varsOfClause *)
+Definition c__varsOfClause := 2.
+Definition varsOfClause_time (c : clause) := map_time (fun _ => c__varsOfLiteral) c + concat_time (map varsOfLiteral c) + c__varsOfClause. 
+Instance term_varsOfClause : computableTime' varsOfClause (fun c _ => (varsOfClause_time c, tt)). 
+Proof. 
+  extract. solverec. unfold varsOfClause_time, c__varsOfClause. solverec. 
+Defined. 
+
+Definition c__varsOfClauseBound1 := (c__varsOfLiteral + 1) * (c__map + 1). 
+Definition c__varsOfClauseBound2 := (c__listsizeCons + c__listsizeNil + 1). 
+Definition poly__varsOfClause n := (n + 1) * c__varsOfClauseBound1 + poly__concat (n * c__varsOfClauseBound2) + c__varsOfClause.
+Lemma varsOfClause_time_bound c : varsOfClause_time c <= poly__varsOfClause (size (enc c)).
+Proof. 
+  unfold varsOfClause_time. 
+  change (fun _ : bool * nat => c__varsOfLiteral) with ((fun _ (_ : bool * nat) => c__varsOfLiteral) tt). 
+  rewrite map_time_bound_env. 
+  2: { 
+    split.
+    - intros. instantiate (1 := registered_unit_enc). instantiate (1 := fun (n : nat) => c__varsOfLiteral). cbn; nia.
+    - smpl_inO. 
+  } 
+  rewrite concat_time_bound. 
+  poly_mono concat_poly. 
+  2: { 
+    instantiate (1 := size (enc c) + (|c|) * (c__listsizeCons + c__listsizeNil)). 
+    induction c; cbn -[Nat.add]; [easy | ].
+    rewrite !list_size_cons. rewrite varsOfLiteral_size, IHc. nia.
+  }
+  unfold poly__varsOfClause, c__varsOfClauseBound1, c__varsOfClauseBound2. 
+  poly_mono concat_poly. 
+  2 : { instantiate (1 := size (enc c) * (c__listsizeCons + c__listsizeNil + 1)). rewrite list_size_length. 
+        nia.
+  }
+  rewrite list_size_length. 
+  nia. 
+Qed. 
+Lemma varsOfClause_poly : monotonic poly__varsOfClause /\ inOPoly poly__varsOfClause. 
+Proof. 
+  split; unfold poly__varsOfClause; smpl_inO. 
+  - apply concat_poly. 
+  - apply inOPoly_comp; [apply concat_poly | apply concat_poly | smpl_inO]. 
 Qed. 
 
-(*some more bounds required for the following inNP proof*)
-Lemma list_bound_enc_size (X : Type) `{registered X} : (exists c, forall (x : X), size(enc x) <= c) -> exists c' c'', forall (l : list X), size(enc l) <= (c' * |l|) + c''. 
-Proof.
-  intros [c H1]. evar (c' : nat). evar (c'' : nat). exists c', c''.  
-  induction l.
-  - instantiate (c'' := 4). subst c''. enough (size(enc ([] : list X)) <= 4) by lia. now cbv. 
-  - rewrite size_list. cbn.
-    rewrite size_list in IHl. rewrite <- Nat.add_assoc. rewrite IHl.
-    solverec. rewrite (H1 a). instantiate (c' := c + 5). subst c'; solverec. 
+(*varsOfCnf *)
+Definition c__varsOfCnf := 2.
+Definition varsOfCnf_time (cn : cnf) := map_time (fun cl => varsOfClause_time cl) cn + concat_time (map varsOfClause cn) + c__varsOfCnf.
+Instance term_varsOfCnf : computableTime' varsOfCnf (fun c _ => (varsOfCnf_time c, tt)). 
+Proof. 
+  extract. solverec. unfold varsOfCnf_time, c__varsOfCnf; solverec. 
+Defined. 
+
+Definition c__varsOfCnfBound := (c__listsizeCons + c__listsizeNil + 1). 
+Definition poly__varsOfCnf n := (n + 1) * (poly__varsOfClause (size (enc tt) + n) + 1) * (c__map + 1) + poly__concat (n * c__varsOfCnfBound + c__listsizeNil) + c__varsOfCnf.
+Lemma varsOfCnf_time_bound c : varsOfCnf_time c <= poly__varsOfCnf (size (enc c)).
+Proof. 
+  unfold varsOfCnf_time. 
+  change (fun cl => varsOfClause_time cl) with ((fun _ cl => varsOfClause_time cl) tt). 
+  rewrite map_time_bound_env. 
+  2: { 
+    split.
+    - intros. instantiate (1 := registered_unit_enc). 
+      rewrite varsOfClause_time_bound. poly_mono varsOfClause_poly. 
+      2: { instantiate (1 := size (enc env) + size (enc ele)); lia. }
+      reflexivity.
+    - apply varsOfClause_poly.
+  } 
+  rewrite concat_time_bound. 
+  poly_mono concat_poly. 
+  2: { 
+    instantiate (1 := (size (enc c) * (c__listsizeCons + c__listsizeNil + 1)) + c__listsizeNil). 
+    induction c; cbn -[Nat.add]; [rewrite size_list; cbn -[Nat.add]; nia | ].
+    rewrite !list_size_cons. rewrite varsOfClause_size, IHc. rewrite list_size_length. nia.
+  }
+  unfold poly__varsOfCnf, c__varsOfCnfBound.
+  rewrite list_size_length. 
+  nia. 
+Qed. 
+Lemma varsOfCnf_poly : monotonic poly__varsOfCnf /\ inOPoly poly__varsOfCnf. 
+Proof. 
+  split; unfold poly__varsOfCnf; smpl_inO. 
+  - apply varsOfClause_poly.
+  - apply concat_poly. 
+  - apply inOPoly_comp; [apply varsOfClause_poly | apply varsOfClause_poly | smpl_inO].
+  - apply inOPoly_comp; [apply concat_poly | apply concat_poly | smpl_inO]. 
 Qed. 
 
-Lemma clause_maxVar_bound_enc (c : clause) : clause_maxVar c <= size(enc c). 
-Proof.
-  induction c. 
-  - cbn. lia.
-  - cbn. destruct a. unfold clause_maxVar in IHc; rewrite IHc. 
-    rewrite list_size_cons, size_prod; cbn [fst snd]. 
-    rewrite max_bound. solverec. rewrite size_nat_enc. solverec. 
-Qed. 
+(*assignment_small_decb *)
+Definition c__assignmentSmallDecb := 17.
+Definition assignment_small_decb_time (cn : cnf) a := varsOfCnf_time cn + list_incl_decb_time (fun x y => c__nat_eqb2 + nat_eqb_time x y) a (varsOfCnf cn) + dupfreeb_time (fun x y => c__nat_eqb2 + nat_eqb_time x y) a + c__assignmentSmallDecb.
+Instance term_assignment_small_decb : computableTime' assignment_small_decb (fun cn _ => (1, fun a _ => (assignment_small_decb_time cn a, tt))). 
+Proof. 
+  extract. solverec. unfold assignment_small_decb_time, c__assignmentSmallDecb. solverec. 
+Defined. 
 
-Lemma cnf_maxVar_bound_enc (c : cnf) : cnf_maxVar c <= size(enc c). 
-Proof.
-  induction c.
-  - cbn; lia.
-  - cbn. unfold cnf_maxVar in IHc; rewrite IHc. 
-    rewrite max_bound.
-    rewrite list_size_cons. rewrite clause_maxVar_bound_enc. solverec. 
+(*we first bound the components separately *)
+Definition c__assignmentSmallDecbBound1 := (1 + c__listsizeCons + c__listsizeNil).
+Definition c__assignmentSmallDecbBound2 := c__nat_eqb2 + c__list_in_decb.
+Definition poly__assignmentSmallDecb1 n := (n + 1) * (n * c__assignmentSmallDecbBound1 + 1) * (c__assignmentSmallDecbBound2 + (n * c__assignmentSmallDecbBound1 + n + size (enc tt) + 1) * c__nat_eqb) + (n + 1) * c__list_incl_decb.
+Lemma assignment_small_decb_time_bound1 a cn: list_incl_decb_time (fun x y => c__nat_eqb2 + nat_eqb_time x y)a (varsOfCnf cn) <= poly__assignmentSmallDecb1 (size (enc cn) + size (enc a)).
+Proof. 
+  change (fun x y => c__nat_eqb2 + nat_eqb_time x y) with ((fun env x y => c__nat_eqb2 + nat_eqb_time x y) tt). 
+  rewrite list_incl_decb_time_bound_env. 
+  2: { 
+    split. 
+    - intros x y env. rewrite nat_eqb_time_bound_l. 
+      instantiate (1 := registered_unit_enc).
+      instantiate (1 := fun n => c__nat_eqb2 + (n + 1) * c__nat_eqb). nia. 
+    - smpl_inO. 
+  }
+  rewrite !list_size_length. rewrite varsOfCnf_size.
+  unfold poly__assignmentSmallDecb1, c__assignmentSmallDecbBound1, c__assignmentSmallDecbBound2.
+
+  (*help nia to achieve an acceptable rt *)
+  replace_le (size (enc a)) with (size (enc cn) + size (enc a)) by lia at 1. 
+  replace_le (size (enc cn)) with (size (enc cn) + size (enc a)) by lia at 2.
+  replace_le (size (enc cn)) with (size (enc cn) + size (enc a)) by lia at 3. 
+  replace_le (size (enc a)) with (size (enc cn) + size (enc a)) by lia at 4. 
+  replace_le (size (enc a)) with (size (enc cn) + size (enc a)) by lia at 5. 
+  generalize (size (enc cn) + size (enc a)). intros n. nia.
 Qed.
+Lemma assignment_small_decb_poly1 : monotonic poly__assignmentSmallDecb1 /\ inOPoly poly__assignmentSmallDecb1. 
+Proof. 
+  unfold poly__assignmentSmallDecb1; split; smpl_inO.
+Qed. 
 
-Lemma sat_NP : inNP SAT.
+Definition poly__assignmentSmallDecb2 n := (n + 1) * (n + 1) * (c__nat_eqb2 + (2 * n + size (enc tt) + 1) * c__nat_eqb + c__dupfreeBound).
+Lemma assignment_small_decb_time_bound2 a : dupfreeb_time (fun x y => c__nat_eqb2 + nat_eqb_time x y) a <= poly__assignmentSmallDecb2 (size (enc a)). 
+Proof. 
+  change (fun x y => c__nat_eqb2 + nat_eqb_time x y) with ((fun env x y => c__nat_eqb2 + nat_eqb_time x y) tt).
+  rewrite dupfreeb_time_bound_env. 
+  2: { 
+    split.
+    - intros x y env. rewrite nat_eqb_time_bound_l. 
+      instantiate (1 := registered_unit_enc).
+      instantiate (1 := fun n => c__nat_eqb2 + (n + 1) * c__nat_eqb). nia. 
+    - smpl_inO. 
+  } 
+  rewrite list_size_length. 
+  unfold poly__assignmentSmallDecb2. nia.
+Qed.
+Lemma assignment_small_decb_poly2 : monotonic poly__assignmentSmallDecb2 /\ inOPoly poly__assignmentSmallDecb2. 
+Proof. 
+  unfold poly__assignmentSmallDecb2; split; smpl_inO.
+Qed.
+ 
+
+Definition c__assignmentSmallDecbBound3 := c__nat_eqb2 + c__dupfreeBound.
+  
+Definition poly__assignmentSmallDecb n := 
+  poly__varsOfCnf n 
+  + poly__assignmentSmallDecb1 n 
+  + poly__assignmentSmallDecb2 n
+  + c__assignmentSmallDecb.
+Lemma assignment_small_decb_time_bound cn a : assignment_small_decb_time cn a <= poly__assignmentSmallDecb (size (enc cn) + size (enc a)). 
+Proof. 
+  unfold assignment_small_decb_time.
+  rewrite varsOfCnf_time_bound. 
+  rewrite assignment_small_decb_time_bound1. 
+  rewrite assignment_small_decb_time_bound2.  
+  poly_mono varsOfCnf_poly. 
+  2: { instantiate (1 := size (enc cn) + size (enc a)); lia. }
+  poly_mono assignment_small_decb_poly2.
+  2: { instantiate (1 := size (enc cn) + size (enc a)); lia. } 
+  unfold poly__assignmentSmallDecb; lia. 
+Qed. 
+
+Lemma assignment_small_decb_poly : monotonic poly__assignmentSmallDecb /\ inOPoly poly__assignmentSmallDecb.
+Proof. 
+  unfold poly__assignmentSmallDecb; split; smpl_inO.
+  3, 6: apply assignment_small_decb_poly2. 
+  2, 4: apply assignment_small_decb_poly1. 
+  1, 2: apply varsOfCnf_poly.
+Qed. 
+
+(*sat_verifierb *)
+Definition c__satVerifierb := 12. 
+Definition sat_verifierb_time (p : cnf * assgn) := match p with (cn, a) => assignment_small_decb_time cn a + evalCnf_time a cn + c__satVerifierb end.
+Instance term_sat_verifierb : computableTime' sat_verifierb (fun p _ => (sat_verifierb_time p, tt)). 
+Proof. 
+  extract. solverec. unfold sat_verifierb_time, c__satVerifierb. solverec. 
+Defined. 
+
+Definition poly__sat_verifierb n := poly__assignmentSmallDecb n + poly__evalCnf n + c__satVerifierb.
+Lemma sat_verifierb_time_bound p : sat_verifierb_time p <= poly__sat_verifierb (size (enc p)). 
+Proof. 
+  unfold sat_verifierb_time. 
+  destruct p as [cn a].
+  rewrite assignment_small_decb_time_bound.
+  rewrite evalCnf_time_bound. 
+  rewrite size_prod; cbn.
+
+  poly_mono assignment_small_decb_poly. 
+  2: { instantiate (1 := size (enc cn) + size (enc a) + 4). lia. }
+  poly_mono evalCnf_poly.
+  2: { instantiate (1 := size (enc cn) + size (enc a) + 4). lia. }
+  unfold poly__sat_verifierb. nia.
+Qed. 
+Lemma sat_verifierb_poly : monotonic poly__sat_verifierb /\ inOPoly poly__sat_verifierb. 
+Proof. 
+  split; unfold poly__sat_verifierb; smpl_inO. 
+  2, 4: apply evalCnf_poly.
+  1, 2: apply assignment_small_decb_poly.
+Qed. 
+
+(** We obtain that SAT is in NP *)
+Lemma sat_NP : inNP (unrestrictedP SAT).
 Proof.
-  apply inNP_intro with (R:= sat_verifier). 
-  4 : {
-    unfold SAT, sat_verifier. intros x; split.
-    - intros [a H]. pose (a' := takeN a (S(cnf_maxVar x))). (*use a shorted assignment*)
-      exists a'. repeat split. apply bounded_cap_assgn_cnf. apply cnf_maxVar_bound. 
-      assumption. apply takeN_length. 
-    - intros (a & H1 &H2). exists a; tauto.
-  }
-  3 : {
-    unfold polyBalanced.
-    destruct (list_bound_enc_size (X:= bool)) as (c' & c'' & H').
-    {exists 5. intros []; cbv; lia. }
-    evar (f : nat -> nat). exists f. split; try split.
-    2: { intros x a (H1 & H2). 
-         (*idea: x contains the maxVar and each entry of a has constant size (booleans)  *)
-         rewrite H'. rewrite H2. solverec. 
-         rewrite cnf_maxVar_bound_enc.
-         generalize (size (enc x)) as n; intros n. 
-         [f]: intros n. subst f. cbn. 
-         reflexivity. 
-    }
-    1-2: subst f; smpl_inO. 
-  }
+  apply inNP_intro with (R:= fun (a : { cnf | True}) => sat_verifier (proj1_sig a)). 
   1 : apply linDec_polyTimeComputable.
+  2 : {
+    exists (fun n => n * (1 + c__listsizeCons + c__listsizeNil)). 
+    3, 4: smpl_inO.
+    - unfold SAT, sat_verifier.
+      intros (cn & ?) a (H1 & H2). cbn. exists a; tauto.  
+    - unfold SAT, sat_verifier. intros (cn & ?) [a H]. exists (compressAssignment a cn). split. 
+      + apply compressAssignment_cnf_equiv in H. cbn. split; [apply H | apply compressAssignment_small]. 
+      + apply assignment_small_size. cbn. apply compressAssignment_small. 
+  }
 
-  destruct (sat_verifierb_time_bound) as (f' & H1 & H2 & H3). 
-  evar (f : nat -> nat). exists f. split.
-  + exists (fun x => sat_verifierb x). split.
-    - constructor. extract. solverec. rewrite H1. rewrite size_prod; cbn [fst snd].  
-      [f]: intros n. subst f; cbn. unfold monotonic in H3.
-      rewrite H3 with (x':= size(enc a) + size(enc b) + 4). 2:lia.
-      generalize (size(enc a) + size(enc b) + 4). intros n; reflexivity. 
-    - intros [cn a]. cbn [prod_curry]. apply (reflect_iff). apply sat_verifierb_correct. 
- + split; subst f; smpl_inO. 
+  unfold inTimePoly. exists poly__sat_verifierb. repeat split.
+  - exists (sat_verifierb). 
+    + eexists. 
+      eapply computesTime_timeLeq. 2: apply term_sat_verifierb.
+      cbn. intros [N a] _. split; [ apply sat_verifierb_time_bound | easy]. 
+    + intros [N a] ?. cbn. apply sat_verifierb_correct.
+  - apply sat_verifierb_poly. 
+  - apply sat_verifierb_poly. 
 Qed. 
