theories/L/Complexity/Problems/FlatClique.v
@@ -2,7 +2,7 @@ From Undecidability.L Require Import L.
 From Undecidability.L.Tactics Require Import LTactics GenEncode.
 From Undecidability.L.Datatypes Require Import LLists LLNat LProd.
 From PslBase Require Import FinTypes. 
-From Undecidability.L.Complexity.Problems Require Import FlatUGraph newClique UGraph.
+From Undecidability.L.Complexity.Problems Require Import FlatUGraph Clique UGraph.
 From Undecidability.L.Complexity.Cook Require Import FlatFinTypes.
 
 Definition isfClique (G : fgraph) (l : list fvertex) := 
